<?xml version="1.0"?>
<rdf:RDF xmlns="http://www.ebi.ac.uk/swo/swo.owl"
     xml:base="http://www.ebi.ac.uk/swo/swo.owl"
     xmlns:dc="http://purl.org/dc/elements/1.1/"
     xmlns:obo="http://purl.obolibrary.org/obo/"
     xmlns:owl="http://www.w3.org/2002/07/owl#"
     xmlns:rdf="http://www.w3.org/1999/02/22-rdf-syntax-ns#"
     xmlns:xml="http://www.w3.org/XML/1998/namespace"
     xmlns:xsd="http://www.w3.org/2001/XMLSchema#"
     xmlns:rdfs="http://www.w3.org/2000/01/rdf-schema#">
    <owl:Ontology rdf:about="http://www.ebi.ac.uk/swo/swo.owl"/>
    


    <!-- 
    ///////////////////////////////////////////////////////////////////////////////////////
    //
    // Annotation properties
    //
    ///////////////////////////////////////////////////////////////////////////////////////
     -->

    


    <!-- http://purl.obolibrary.org/obo/IAO_0000115 -->

    <owl:AnnotationProperty rdf:about="http://purl.obolibrary.org/obo/IAO_0000115"/>
    


    <!-- http://purl.obolibrary.org/obo/IAO_0000118 -->

    <owl:AnnotationProperty rdf:about="http://purl.obolibrary.org/obo/IAO_0000118"/>
    


    <!-- http://purl.obolibrary.org/obo/IAO_0000119 -->

    <owl:AnnotationProperty rdf:about="http://purl.obolibrary.org/obo/IAO_0000119"/>
    


    <!-- http://purl.org/dc/elements/1.1/contributor -->

    <owl:AnnotationProperty rdf:about="http://purl.org/dc/elements/1.1/contributor"/>
    


    <!-- http://purl.org/dc/elements/1.1/creator -->

    <owl:AnnotationProperty rdf:about="http://purl.org/dc/elements/1.1/creator"/>
    


    <!-- 
    ///////////////////////////////////////////////////////////////////////////////////////
    //
    // Classes
    //
    ///////////////////////////////////////////////////////////////////////////////////////
     -->

    


    <!-- http://www.ebi.ac.uk/swo/SWO_0000002 -->

    <owl:Class rdf:about="http://www.ebi.ac.uk/swo/SWO_0000002">
        <obo:IAO_0000115>A license is a legal instrument (usually by way of contract law, with or without printed material) governing the use or redistribution of the resource containing the license.</obo:IAO_0000115>
        <obo:IAO_0000119>Modified from http://en.wikipedia.org/wiki/Software_license</obo:IAO_0000119>
        <dc:creator>James Malone</dc:creator>
        <rdfs:label xml:lang="en">license</rdfs:label>
        <rdfs:label>software license</rdfs:label>
    </owl:Class>
    


    <!-- http://www.ebi.ac.uk/swo/license/SWO_1000001 -->

    <owl:Class rdf:about="http://www.ebi.ac.uk/swo/license/SWO_1000001">
        <rdfs:subClassOf rdf:resource="http://www.ebi.ac.uk/swo/SWO_0000002"/>
        <obo:IAO_0000118>CC</obo:IAO_0000118>
        <rdfs:label>Creative Commons</rdfs:label>
    </owl:Class>
    


    <!-- http://www.ebi.ac.uk/swo/license/SWO_1000002 -->

    <owl:Class rdf:about="http://www.ebi.ac.uk/swo/license/SWO_1000002">
        <rdfs:subClassOf rdf:resource="http://www.ebi.ac.uk/swo/SWO_0000002"/>
        <rdfs:label>Proprietary commercial software license</rdfs:label>
    </owl:Class>
    


    <!-- http://www.ebi.ac.uk/swo/license/SWO_1000003 -->

    <owl:Class rdf:about="http://www.ebi.ac.uk/swo/license/SWO_1000003">
        <rdfs:subClassOf rdf:resource="http://www.ebi.ac.uk/swo/license/SWO_9000088"/>
        <obo:IAO_0000118>Mozilla Public License Version 1.1</obo:IAO_0000118>
        <rdfs:label>MPL v1.1</rdfs:label>
    </owl:Class>
    


    <!-- http://www.ebi.ac.uk/swo/license/SWO_1000004 -->

    <owl:Class rdf:about="http://www.ebi.ac.uk/swo/license/SWO_1000004">
        <rdfs:subClassOf rdf:resource="http://www.ebi.ac.uk/swo/license/SWO_1000043"/>
        <obo:IAO_0000118>GNU General Public License</obo:IAO_0000118>
        <rdfs:label>GNU GPL</rdfs:label>
    </owl:Class>
    


    <!-- http://www.ebi.ac.uk/swo/license/SWO_1000005 -->

    <owl:Class rdf:about="http://www.ebi.ac.uk/swo/license/SWO_1000005">
        <rdfs:subClassOf rdf:resource="http://www.ebi.ac.uk/swo/license/SWO_1000009"/>
        <rdfs:subClassOf rdf:resource="http://www.ebi.ac.uk/swo/license/SWO_1000044"/>
        <obo:IAO_0000115>This is a free software license under the definition of &quot;free&quot; by the GNU Project, and is compatible with version 3 of the GNU GPL.</obo:IAO_0000115>
        <obo:IAO_0000119>http://www.gnu.org/licenses/license-list.html, accessed 12 June 2013.</obo:IAO_0000119>
        <dc:creator>Allyson Lister</dc:creator>
        <rdfs:label>Apache License Version 2.0</rdfs:label>
    </owl:Class>
    


    <!-- http://www.ebi.ac.uk/swo/license/SWO_1000006 -->

    <owl:Class rdf:about="http://www.ebi.ac.uk/swo/license/SWO_1000006">
        <rdfs:subClassOf rdf:resource="http://www.ebi.ac.uk/swo/license/SWO_1000043"/>
        <obo:IAO_0000115>The Academic Free License is a free software license under the definition of &quot;free&quot; by the GNU Project, is not copyleft, and is incompatible with the GNU GPL.</obo:IAO_0000115>
        <obo:IAO_0000118>AFL</obo:IAO_0000118>
        <obo:IAO_0000119>http://directory.fsf.org/wiki/License:AFLv3, accessed 12 June 2013; http://www.gnu.org/licenses/license-list.html, accessed 12 June 2013</obo:IAO_0000119>
        <dc:creator>Allyson Lister</dc:creator>
        <dc:creator>Andy Brown</dc:creator>
        <rdfs:label>Academic Free License version 3</rdfs:label>
    </owl:Class>
    


    <!-- http://www.ebi.ac.uk/swo/license/SWO_1000007 -->

    <owl:Class rdf:about="http://www.ebi.ac.uk/swo/license/SWO_1000007">
        <rdfs:subClassOf rdf:resource="http://www.ebi.ac.uk/swo/license/SWO_1000044"/>
        <obo:IAO_0000115>This is the original BSD license with the advertising clause and another clause removed. (It is also sometimes called the “2-clause BSD license”.) It is a lax, permissive non-copyleft free software license, compatible with the GNU GPL.</obo:IAO_0000115>
        <obo:IAO_0000118>2-clause BSD License</obo:IAO_0000118>
        <obo:IAO_0000119>http://www.gnu.org/licenses/license-list.html, accessed 12 June 2013.</obo:IAO_0000119>
        <dc:creator>Allyson Lister</dc:creator>
        <dc:creator>Andy Brown</dc:creator>
        <rdfs:label>FreeBSD</rdfs:label>
    </owl:Class>
    


    <!-- http://www.ebi.ac.uk/swo/license/SWO_1000008 -->

    <owl:Class rdf:about="http://www.ebi.ac.uk/swo/license/SWO_1000008">
        <rdfs:subClassOf rdf:resource="http://www.ebi.ac.uk/swo/SWO_0000002"/>
        <rdfs:label>Open source software license</rdfs:label>
    </owl:Class>
    


    <!-- http://www.ebi.ac.uk/swo/license/SWO_1000009 -->

    <owl:Class rdf:about="http://www.ebi.ac.uk/swo/license/SWO_1000009">
        <rdfs:subClassOf rdf:resource="http://www.ebi.ac.uk/swo/SWO_0000002"/>
        <rdfs:label>License without restrictions on derivatives</rdfs:label>
    </owl:Class>
    


    <!-- http://www.ebi.ac.uk/swo/license/SWO_1000043 -->

    <owl:Class rdf:about="http://www.ebi.ac.uk/swo/license/SWO_1000043">
        <rdfs:subClassOf rdf:resource="http://www.ebi.ac.uk/swo/license/SWO_1000008"/>
        <obo:IAO_0000115>A licensed is a free license according to GNU if the users have the four essential freedoms:

    The freedom to run the program, for any purpose (freedom 0).
    The freedom to study how the program works, and change it so it does your computing as you wish (freedom 1). Access to the source code is a precondition for this.
    The freedom to redistribute copies so you can help your neighbor (freedom 2).
    The freedom to distribute copies of your modified versions to others (freedom 3). By doing this you can give the whole community a chance to benefit from your changes. Access to the source code is a precondition for this.

A program is free software if users have all of these freedoms. Thus, you should be free to redistribute copies, either with or without modifications, either gratis or charging a fee for distribution, to anyone anywhere. Being free to do these things means (among other things) that you do not have to ask or pay for permission to do so. 

“Free software” does not mean “noncommercial”. A free program must be available for commercial use, commercial development, and commercial distribution. Commercial development of free software is no longer unusual; such free commercial software is very important. You may have paid money to get copies of free software, or you may have obtained copies at no charge. But regardless of how you got your copies, you always have the freedom to copy and change the software, even to sell copies. </obo:IAO_0000115>
        <obo:IAO_0000119>http://www.gnu.org/philosophy/free-sw.html, accessed 12 June 2013.</obo:IAO_0000119>
        <dc:creator>Allyson Lister</dc:creator>
        <rdfs:comment>Allyson Lister: This class defines those licenses which are free licenses, but which may or may not be compatible with any version of the GNU GPL.</rdfs:comment>
        <rdfs:label>GNU Project Free License Type</rdfs:label>
    </owl:Class>
    


    <!-- http://www.ebi.ac.uk/swo/license/SWO_1000044 -->

    <owl:Class rdf:about="http://www.ebi.ac.uk/swo/license/SWO_1000044">
        <rdfs:subClassOf rdf:resource="http://www.ebi.ac.uk/swo/license/SWO_1000043"/>
        <obo:IAO_0000115>GNU GPL Compatible License Type is a GNU Project Free License Type which is also compatible with one or more versions of the GNU GPL</obo:IAO_0000115>
        <obo:IAO_0000119>Modified from http://www.gnu.org/copyleft/copyleft.html, accessed 12 June 2013.</obo:IAO_0000119>
        <dc:creator>Allyson Lister</dc:creator>
        <rdfs:label>GNU GPL Compatible License Type</rdfs:label>
    </owl:Class>
    


    <!-- http://www.ebi.ac.uk/swo/license/SWO_1000046 -->

    <owl:Class rdf:about="http://www.ebi.ac.uk/swo/license/SWO_1000046">
        <rdfs:subClassOf rdf:resource="http://www.ebi.ac.uk/swo/license/SWO_1000004"/>
        <obo:IAO_0000115>The GNU GPL v3 is the latest version of the GNU GPL: a free software license, and a copyleft license. Please note that GPLv3 is not compatible with GPLv2 by itself. However, most software released under GPLv2 allows you to use the terms of later versions of the GPL as well. When this is the case, you can use the code under GPLv3 to make the desired combination.</obo:IAO_0000115>
        <obo:IAO_0000118>GNU General Public License Version 3</obo:IAO_0000118>
        <obo:IAO_0000119>https://www.gnu.org/licenses/license-list.html, accessed on 23 June 2016.</obo:IAO_0000119>
        <dc:creator>Allyson Lister</dc:creator>
        <rdfs:label xml:lang="en">GNU GPL v3</rdfs:label>
    </owl:Class>
    


    <!-- http://www.ebi.ac.uk/swo/license/SWO_1000047 -->

    <owl:Class rdf:about="http://www.ebi.ac.uk/swo/license/SWO_1000047">
        <rdfs:subClassOf rdf:resource="http://www.ebi.ac.uk/swo/license/SWO_1000004"/>
        <obo:IAO_0000115>The GNU GPL v2 is an earlier version of the GNU GPL: a free software license, and a copyleft license. Please note that GPLv2 is, by itself, not compatible with GPLv3. However, most software released under GPLv2 allows you to use the terms of later versions of the GPL as well. When this is the case, you can use the code under GPLv3 to make the desired combination.</obo:IAO_0000115>
        <obo:IAO_0000118>GNU General Public License Version 2</obo:IAO_0000118>
        <obo:IAO_0000119>https://www.gnu.org/licenses/license-list.html, accessed 23 June 2016.</obo:IAO_0000119>
        <rdfs:label xml:lang="en">GNU GPL v2</rdfs:label>
    </owl:Class>
    


    <!-- http://www.ebi.ac.uk/swo/license/SWO_1000049 -->

    <owl:Class rdf:about="http://www.ebi.ac.uk/swo/license/SWO_1000049">
        <rdfs:subClassOf rdf:resource="http://www.ebi.ac.uk/swo/license/SWO_1000001"/>
        <rdfs:subClassOf rdf:resource="http://www.ebi.ac.uk/swo/license/SWO_1000009"/>
        <rdfs:subClassOf rdf:resource="http://www.ebi.ac.uk/swo/license/SWO_1000044"/>
        <obo:IAO_0000115>CC0 is a public domain dedication from Creative Commons. A work released under CC0 is dedicated to the public domain to the fullest extent permitted by law. If that is not possible for any reason, CC0 also provides a lax, permissive license as a fallback. Both public domain works and the lax license provided by CC0 are compatible with the GNU GPL.</obo:IAO_0000115>
        <obo:IAO_0000118>CC0 1.0 Universal (CC0 1.0) Public Domain Dedication</obo:IAO_0000118>
        <obo:IAO_0000119>http://www.gnu.org/licenses/license-list.html, accessed 12 June 2013.</obo:IAO_0000119>
        <dc:creator>Allyson Lister</dc:creator>
        <rdfs:label>CC0 1.0</rdfs:label>
    </owl:Class>
    


    <!-- http://www.ebi.ac.uk/swo/license/SWO_1000050 -->

    <owl:Class rdf:about="http://www.ebi.ac.uk/swo/license/SWO_1000050">
        <rdfs:subClassOf rdf:resource="http://www.ebi.ac.uk/swo/license/SWO_1000001"/>
        <rdfs:subClassOf rdf:resource="http://www.ebi.ac.uk/swo/license/SWO_1000044"/>
        <obo:IAO_0000115>CC BY 2.0 is a non-copyleft free (free by the definition of the GNU Project) license which lets others distribute, remix, tweak, and build upon your work, even commercially, as long as they credit you for the original creation. This is the most accommodating of Creative Commons licenses offered. Recommended for maximum dissemination and use of licensed materials. The GNU Project recommend it for art, entertainment works, and educational works. It is compatible with all versions of the GNU GPL; however, like all CC licenses, it should not be used on software.</obo:IAO_0000115>
        <obo:IAO_0000118>Creative Commons Attribution 2.0 Generic (CC BY 2.0)</obo:IAO_0000118>
        <obo:IAO_0000119>Modified from http://www.gnu.org/licenses/license-list.html, accessed 12 June 2013 and 28 June 2016; Modified from http://creativecommons.org/licenses/, accessed 12 June 2013.</obo:IAO_0000119>
        <dc:creator>Allyson Lister</dc:creator>
        <rdfs:label xml:lang="en">CC BY 2.0</rdfs:label>
    </owl:Class>
    


    <!-- http://www.ebi.ac.uk/swo/license/SWO_1000052 -->

    <owl:Class rdf:about="http://www.ebi.ac.uk/swo/license/SWO_1000052">
        <rdfs:subClassOf rdf:resource="http://www.ebi.ac.uk/swo/license/SWO_1000001"/>
        <rdfs:subClassOf rdf:resource="http://www.ebi.ac.uk/swo/license/SWO_1000043"/>
        <obo:IAO_0000115>CC BY-SA 2.0 is a copyleft free (free by the definition of the GNU Project) license which lets others remix, tweak, and build upon your work even for commercial purposes, as long as they credit you and license their new creations under the identical terms. The GNU Project recommend this license for art, entertainment and educational works, but also recommend that it is not used for software or documentation, since it is tricky as to how exactly this license is compatible with the GNU GPL.</obo:IAO_0000115>
        <obo:IAO_0000118>Creative Commons Attribution-Sharealike 2.0 Generic</obo:IAO_0000118>
        <obo:IAO_0000119>Modified from http://www.gnu.org/licenses/license-list.html, accessed 12 June 2013; Modified from http://creativecommons.org/licenses/, accessed 12 June 2013.</obo:IAO_0000119>
        <dc:creator>Allyson Lister</dc:creator>
        <rdfs:label>CC BY-SA 2.0</rdfs:label>
    </owl:Class>
    


    <!-- http://www.ebi.ac.uk/swo/license/SWO_1000053 -->

    <owl:Class rdf:about="http://www.ebi.ac.uk/swo/license/SWO_1000053">
        <rdfs:subClassOf rdf:resource="http://www.ebi.ac.uk/swo/license/SWO_9000086"/>
        <obo:IAO_0000115>LPPL v1.3 is a free software license (by the defintion of the GNU Project), with less stringent requirements on distribution than LPPL 1.2. It is still incompatible with the GPL because some modified versions must include a copy of or pointer to an unmodified version.Software projects other than LaTeX rarely use it.</obo:IAO_0000115>
        <obo:IAO_0000118 xml:lang="en">Latex Project Public License v1.3c</obo:IAO_0000118>
        <obo:IAO_0000119>Modified from http://en.wikipedia.org/wiki/LaTeX_Project_Public_License, accessed 12 June 2013; modified from http://www.gnu.org/licenses/license-list.html, accessed 12 June 2013.</obo:IAO_0000119>
        <rdfs:label>LPPL v1.3c</rdfs:label>
    </owl:Class>
    


    <!-- http://www.ebi.ac.uk/swo/license/SWO_1000054 -->

    <owl:Class rdf:about="http://www.ebi.ac.uk/swo/license/SWO_1000054">
        <rdfs:subClassOf rdf:resource="http://www.ebi.ac.uk/swo/license/SWO_9000086"/>
        <obo:IAO_0000115>LPPL v1.2 is a free software license (by the defintion of the GNU Project), This license is an incomplete statement of the distribution terms for LaTeX. While it is a free software license, it is incompatible with the GPL because it has many requirements that are not in the GPL. Software projects other than LaTeX rarely use it.</obo:IAO_0000115>
        <obo:IAO_0000118 xml:lang="en">Latex Project Public License v1.2</obo:IAO_0000118>
        <obo:IAO_0000119>Modified from http://en.wikipedia.org/wiki/LaTeX_Project_Public_License, accessed 12 June 2013; modified from http://www.gnu.org/licenses/license-list.html, accessed 12 June 2013.</obo:IAO_0000119>
        <rdfs:label xml:lang="en">LPPL v1.2</rdfs:label>
    </owl:Class>
    


    <!-- http://www.ebi.ac.uk/swo/license/SWO_1000055 -->

    <owl:Class rdf:about="http://www.ebi.ac.uk/swo/license/SWO_1000055">
        <rdfs:subClassOf rdf:resource="http://www.ebi.ac.uk/swo/license/SWO_1000044"/>
        <rdfs:subClassOf rdf:resource="http://www.ebi.ac.uk/swo/license/SWO_9000088"/>
        <obo:IAO_0000115>MPL v2.0 a free software license as defined by the GNU Project. Section 3.3 provides indirect compatibility between this license and the GNU GPL version 2.0, the GNU LGPL version 2.1, the GNU AGPL version 3.0, and all later versions of those licenses. The MPL allows covered source code to be mixed with other files under a different, even proprietary license. However, code files licensed under the MPL must remain under the MPL and freely available in source form.</obo:IAO_0000115>
        <obo:IAO_0000119>http://www.gnu.org/licenses/license-list.html, accessed 12 June 2013; http://en.wikipedia.org/wiki/Mozilla_Public_License, accessed 12 June 2013.</obo:IAO_0000119>
        <rdfs:label xml:lang="en">MPL v2.0</rdfs:label>
        <rdfs:label>Mozilla Public License Version 2.0</rdfs:label>
    </owl:Class>
    


    <!-- http://www.ebi.ac.uk/swo/license/SWO_1000056 -->

    <owl:Class rdf:about="http://www.ebi.ac.uk/swo/license/SWO_1000056">
        <rdfs:subClassOf rdf:resource="http://www.ebi.ac.uk/swo/SWO_0000002"/>
        <dc:creator>Allyson Lister</dc:creator>
        <rdfs:label>Artistic License</rdfs:label>
    </owl:Class>
    


    <!-- http://www.ebi.ac.uk/swo/license/SWO_1000057 -->

    <owl:Class rdf:about="http://www.ebi.ac.uk/swo/license/SWO_1000057">
        <rdfs:subClassOf rdf:resource="http://www.ebi.ac.uk/swo/license/SWO_1000044"/>
        <rdfs:subClassOf rdf:resource="http://www.ebi.ac.uk/swo/license/SWO_1000056"/>
        <obo:IAO_0000115>The Artistic License v 2.0 is a free software license by the definition of the GNU Project and compatible with the GPL thanks to the relicensing option in section 4(c)(ii) (as compared with the Artistic License 1.0).</obo:IAO_0000115>
        <obo:IAO_0000119>http://www.gnu.org/licenses/license-list.html, accessed 12 June 2013.</obo:IAO_0000119>
        <dc:creator>Allyson Lister</dc:creator>
        <rdfs:label>Artistic License 2.0</rdfs:label>
    </owl:Class>
    


    <!-- http://www.ebi.ac.uk/swo/license/SWO_1000061 -->

    <owl:Class rdf:about="http://www.ebi.ac.uk/swo/license/SWO_1000061">
        <rdfs:subClassOf rdf:resource="http://www.ebi.ac.uk/swo/SWO_0000002"/>
        <obo:IAO_0000115>A license which allows any form of usage of the artifact.</obo:IAO_0000115>
        <rdfs:label xml:lang="en">free to use license</rdfs:label>
    </owl:Class>
    


    <!-- http://www.ebi.ac.uk/swo/license/SWO_1000065 -->

    <owl:Class rdf:about="http://www.ebi.ac.uk/swo/license/SWO_1000065">
        <rdfs:subClassOf rdf:resource="http://www.ebi.ac.uk/swo/license/SWO_1000001"/>
        <rdfs:subClassOf rdf:resource="http://www.ebi.ac.uk/swo/license/SWO_1000044"/>
        <obo:IAO_0000115>The CC BY 4.0 license is a Creative Commons license. This is a non-copyleft free license that is good for art and entertainment works, and educational works. It is compatible with all versions of the GNU GPL; however, like all CC licenses, it should not be used on software. People are free to:
Share — copy and redistribute the material in any medium or format;
Adapt — remix, transform, and build upon the material for any purpose, even commercially.
The licensor cannot revoke these freedoms as long as you follow the license terms.
But they must conform to the following terms:
Attribution — You must give appropriate credit, provide a link to the license, and indicate if changes were made. You may do so in any reasonable manner, but not in any way that suggests the licensor endorses you or your use.
No additional restrictions — You may not apply legal terms or technological measures that legally restrict others from doing anything the license permits.</obo:IAO_0000115>
        <obo:IAO_0000118>Creative Commons Attribution 4.0 International (CC BY 4.0)</obo:IAO_0000118>
        <obo:IAO_0000119>http://creativecommons.org/licenses/by/4.0/ accessed June 22, 2016; https://www.gnu.org/licenses/license-list.html, accessed on June 28, 2016.</obo:IAO_0000119>
        <dc:creator>Allyson Lister</dc:creator>
        <rdfs:comment>Allyson Lister: The only restriction on derivatives is that of the attribution requirement. </rdfs:comment>
        <rdfs:label xml:lang="en">CC BY 4.0</rdfs:label>
    </owl:Class>
    


    <!-- http://www.ebi.ac.uk/swo/license/SWO_1000067 -->

    <owl:Class rdf:about="http://www.ebi.ac.uk/swo/license/SWO_1000067">
        <rdfs:subClassOf rdf:resource="http://www.ebi.ac.uk/swo/license/SWO_1000001"/>
        <rdfs:subClassOf rdf:resource="http://www.ebi.ac.uk/swo/license/SWO_1000044"/>
        <obo:IAO_0000115>CC BY 2.0 UK is a UK-specific non-copyleft free (free by the definition of the GNU Project) license which lets others distribute, remix, tweak, and build upon your work, even commercially, as long as they credit you for the original creation. This is the most accommodating of Creative Commons licenses offered. Recommended for maximum dissemination and use of licensed materials. The GNU Project recommend it for art, entertainment works, and educational works. It is compatible with all versions of the GNU GPL; however, like all CC licenses, it should not be used on software.</obo:IAO_0000115>
        <obo:IAO_0000118>Creative Commons Attribution 2.0 UK: England &amp; Wales (CC BY 2.0 UK)</obo:IAO_0000118>
        <obo:IAO_0000119>Modified from the definition of http://www.ebi.ac.uk/swo/license/SWO_1000050.</obo:IAO_0000119>
        <dc:creator>Allyson Lister</dc:creator>
        <rdfs:label xml:lang="en">CC BY 2.0 UK</rdfs:label>
    </owl:Class>
    


    <!-- http://www.ebi.ac.uk/swo/license/SWO_1000068 -->

    <owl:Class rdf:about="http://www.ebi.ac.uk/swo/license/SWO_1000068">
        <rdfs:subClassOf rdf:resource="http://www.ebi.ac.uk/swo/license/SWO_1000044"/>
        <rdfs:subClassOf rdf:resource="http://www.ebi.ac.uk/swo/license/SWO_9000080"/>
        <obo:IAO_0000115>This is the latest version of the LGPL: a free software license, but not a strong copyleft license, because it permits linking with nonfree modules. It is compatible with GPLv3. It is therefore recommend for special circumstances only.

Please note that LGPLv3 is not compatible with GPLv2 by itself. However, most software released under GPLv2 allows you to use the terms of later versions of the GPL as well. When this is the case, you can use the code under GPLv3 to make the desired combination.</obo:IAO_0000115>
        <obo:IAO_0000118>GNU Lesser General Public License (LGPL) version 3 </obo:IAO_0000118>
        <obo:IAO_0000119>https://www.gnu.org/licenses/license-list.html, accessed 23 June 2016.</obo:IAO_0000119>
        <rdfs:label>GNU LGPL v3</rdfs:label>
    </owl:Class>
    


    <!-- http://www.ebi.ac.uk/swo/license/SWO_1000069 -->

    <owl:Class rdf:about="http://www.ebi.ac.uk/swo/license/SWO_1000069">
        <rdfs:subClassOf rdf:resource="http://www.ebi.ac.uk/swo/SWO_0000002"/>
        <rdfs:label xml:lang="en">GNU AGPL</rdfs:label>
    </owl:Class>
    


    <!-- http://www.ebi.ac.uk/swo/license/SWO_1000070 -->

    <owl:Class rdf:about="http://www.ebi.ac.uk/swo/license/SWO_1000070">
        <rdfs:subClassOf rdf:resource="http://www.ebi.ac.uk/swo/license/SWO_1000044"/>
        <rdfs:subClassOf rdf:resource="http://www.ebi.ac.uk/swo/license/SWO_1000069"/>
        <obo:IAO_0000115>This is a free software, copyleft license. Its terms effectively consist of the terms of GPLv3, with an additional paragraph in section 13 to allow users who interact with the licensed software over a network to receive the source for that program. It is recommended that developers consider using the GNU AGPL for any software which will commonly be run over a network.</obo:IAO_0000115>
        <obo:IAO_0000118>GNU Affero General Public License (AGPL) version 3</obo:IAO_0000118>
        <obo:IAO_0000119>https://www.gnu.org/licenses/license-list.html, accessed on 23 June 2016.</obo:IAO_0000119>
        <dc:creator>Allyson Lister</dc:creator>
        <rdfs:label xml:lang="en">GNU AGPL v3</rdfs:label>
    </owl:Class>
    


    <!-- http://www.ebi.ac.uk/swo/license/SWO_1000071 -->

    <owl:Class rdf:about="http://www.ebi.ac.uk/swo/license/SWO_1000071">
        <rdfs:subClassOf rdf:resource="http://www.ebi.ac.uk/swo/license/SWO_1000044"/>
        <rdfs:subClassOf rdf:resource="http://www.ebi.ac.uk/swo/license/SWO_9000080"/>
        <obo:IAO_0000115>This is the previous version of the LGPL: a free software license, but not a strong copyleft license, because it permits linking with nonfree modules. It is compatible with GPLv2 and GPLv3. We generally recommend the latest version of the LGPL, for special circumstances only.</obo:IAO_0000115>
        <obo:IAO_0000118>GNU Lesser General Public License (LGPL) version 2.1</obo:IAO_0000118>
        <obo:IAO_0000119>https://www.gnu.org/licenses/license-list.html, accessed 28 June 2016.</obo:IAO_0000119>
        <rdfs:label xml:lang="en">GNU LGPL v2.1</rdfs:label>
    </owl:Class>
    


    <!-- http://www.ebi.ac.uk/swo/license/SWO_1000072 -->

    <owl:Class rdf:about="http://www.ebi.ac.uk/swo/license/SWO_1000072">
        <rdfs:subClassOf rdf:resource="http://www.ebi.ac.uk/swo/license/SWO_1000001"/>
        <rdfs:subClassOf rdf:resource="http://www.ebi.ac.uk/swo/license/SWO_1000044"/>
        <obo:IAO_0000115>CC BY 2.1 JP is a Japan-specific non-copyleft free (free by the definition of the GNU Project) license which lets others distribute, remix, tweak, and build upon your work, even commercially, as long as they credit you for the original creation. This is the most accommodating of Creative Commons licenses offered. Recommended for maximum dissemination and use of licensed materials. The GNU Project recommend it for art, entertainment works, and educational works. It is compatible with all versions of the GNU GPL; however, like all CC licenses, it should not be used on software.</obo:IAO_0000115>
        <obo:IAO_0000118>Creative Commons Attribution 2.1 Japan (CC BY 2.1 JP)</obo:IAO_0000118>
        <obo:IAO_0000119>Modified from the definition of http://www.ebi.ac.uk/swo/license/SWO_1000050.</obo:IAO_0000119>
        <dc:creator>Allyson Lister</dc:creator>
        <rdfs:label>CC BY 2.1 JP</rdfs:label>
    </owl:Class>
    


    <!-- http://www.ebi.ac.uk/swo/license/SWO_1000073 -->

    <owl:Class rdf:about="http://www.ebi.ac.uk/swo/license/SWO_1000073">
        <rdfs:subClassOf rdf:resource="http://www.ebi.ac.uk/swo/license/SWO_1000001"/>
        <rdfs:subClassOf rdf:resource="http://www.ebi.ac.uk/swo/license/SWO_1000044"/>
        <obo:IAO_0000115>CC BY 2.5 is a non-copyleft free (free by the definition of the GNU Project) license which lets others distribute, remix, tweak, and build upon your work, even commercially, as long as they credit you for the original creation. This is the most accommodating of Creative Commons licenses offered. Recommended for maximum dissemination and use of licensed materials. The GNU Project recommend it for art, entertainment works, and educational works. It is compatible with all versions of the GNU GPL; however, like all CC licenses, it should not be used on software.</obo:IAO_0000115>
        <obo:IAO_0000118>Creative Commons Attribution 2.5 Generic (CC BY 2.5)</obo:IAO_0000118>
        <obo:IAO_0000119>Modified from the definition of http://www.ebi.ac.uk/swo/license/SWO_1000050.</obo:IAO_0000119>
        <dc:creator>Allyson Lister</dc:creator>
        <rdfs:label xml:lang="en">CC BY 2.5</rdfs:label>
    </owl:Class>
    


    <!-- http://www.ebi.ac.uk/swo/license/SWO_1000074 -->

    <owl:Class rdf:about="http://www.ebi.ac.uk/swo/license/SWO_1000074">
        <rdfs:subClassOf rdf:resource="http://www.ebi.ac.uk/swo/license/SWO_1000001"/>
        <rdfs:subClassOf rdf:resource="http://www.ebi.ac.uk/swo/license/SWO_1000044"/>
        <obo:IAO_0000115>CC BY 3.0 AU is an Australia-specific non-copyleft free (free by the definition of the GNU Project) license which lets others distribute, remix, tweak, and build upon your work, even commercially, as long as they credit you for the original creation. This is the most accommodating of Creative Commons licenses offered. Recommended for maximum dissemination and use of licensed materials. The GNU Project recommend it for art, entertainment works, and educational works. It is compatible with all versions of the GNU GPL; however, like all CC licenses, it should not be used on software.</obo:IAO_0000115>
        <obo:IAO_0000118>Creative Commons Attribution 3.0 Australia (CC BY 3.0 AU)</obo:IAO_0000118>
        <obo:IAO_0000119>Modified from the definition of http://www.ebi.ac.uk/swo/license/SWO_1000050.</obo:IAO_0000119>
        <dc:creator>Allyson Lister</dc:creator>
        <rdfs:label xml:lang="en">CC BY 3.0 AU</rdfs:label>
    </owl:Class>
    


    <!-- http://www.ebi.ac.uk/swo/license/SWO_1000075 -->

    <owl:Class rdf:about="http://www.ebi.ac.uk/swo/license/SWO_1000075">
        <rdfs:subClassOf rdf:resource="http://www.ebi.ac.uk/swo/license/SWO_1000001"/>
        <rdfs:subClassOf rdf:resource="http://www.ebi.ac.uk/swo/license/SWO_1000044"/>
        <obo:IAO_0000115>CC BY 3.0 is a non-copyleft free (free by the definition of the GNU Project) license which lets others distribute, remix, tweak, and build upon your work, even commercially, as long as they credit you for the original creation. This is the most accommodating of Creative Commons licenses offered. Recommended for maximum dissemination and use of licensed materials. The GNU Project recommend it for art, entertainment works, and educational works. It is compatible with all versions of the GNU GPL; however, like all CC licenses, it should not be used on software.</obo:IAO_0000115>
        <obo:IAO_0000118>Creative Commons Attribution 3.0 Unported (CC BY 3.0)</obo:IAO_0000118>
        <obo:IAO_0000119>Modified from the definition of http://www.ebi.ac.uk/swo/license/SWO_1000050.</obo:IAO_0000119>
        <dc:creator>Allyson Lister</dc:creator>
        <rdfs:label xml:lang="en">CC BY 3.0</rdfs:label>
    </owl:Class>
    


    <!-- http://www.ebi.ac.uk/swo/license/SWO_1000076 -->

    <owl:Class rdf:about="http://www.ebi.ac.uk/swo/license/SWO_1000076">
        <rdfs:subClassOf rdf:resource="http://www.ebi.ac.uk/swo/license/SWO_1000001"/>
        <rdfs:subClassOf rdf:resource="http://www.ebi.ac.uk/swo/license/SWO_1000044"/>
        <obo:IAO_0000115>CC BY 3.0 US is a US-specific non-copyleft free (free by the definition of the GNU Project) license which lets others distribute, remix, tweak, and build upon your work, even commercially, as long as they credit you for the original creation. This is the most accommodating of Creative Commons licenses offered. Recommended for maximum dissemination and use of licensed materials. The GNU Project recommend it for art, entertainment works, and educational works. It is compatible with all versions of the GNU GPL; however, like all CC licenses, it should not be used on software.</obo:IAO_0000115>
        <obo:IAO_0000118>Creative Commons Attribution 3.0 United States (CC BY 3.0 US)</obo:IAO_0000118>
        <obo:IAO_0000119>Modified from the definition of http://www.ebi.ac.uk/swo/license/SWO_1000050.</obo:IAO_0000119>
        <dc:creator>Allyson Lister</dc:creator>
        <rdfs:label xml:lang="en">CC BY 3.0 US</rdfs:label>
    </owl:Class>
    


    <!-- http://www.ebi.ac.uk/swo/license/SWO_1000077 -->

    <owl:Class rdf:about="http://www.ebi.ac.uk/swo/license/SWO_1000077">
        <rdfs:subClassOf rdf:resource="http://www.ebi.ac.uk/swo/license/SWO_1000001"/>
        <obo:IAO_0000115>CC BY-ND 3.0 is a nonfree license, as there are restrictions on distributing modified versions. You must give appropriate credit, provide a link to the license, and indicate if changes were made. You may do so in any reasonable manner, but not in any way that suggests the licensor endorses you or your use. If you remix, transform, or build upon the material, you may not distribute the modified material. This license is generally used for documentation.</obo:IAO_0000115>
        <obo:IAO_0000118>Creative Commons Attribution-NoDerivs 3.0 Unported (CC BY-ND 3.0)</obo:IAO_0000118>
        <obo:IAO_0000119>https://www.gnu.org/licenses/license-list.html accessed 29 June 2016; https://creativecommons.org/licenses/by-nd/3.0/ accessed 29 June 2016.</obo:IAO_0000119>
        <dc:creator>Allyson Lister</dc:creator>
        <rdfs:label xml:lang="en">CC BY-ND 3.0</rdfs:label>
    </owl:Class>
    


    <!-- http://www.ebi.ac.uk/swo/license/SWO_1000078 -->

    <owl:Class rdf:about="http://www.ebi.ac.uk/swo/license/SWO_1000078">
        <rdfs:subClassOf rdf:resource="http://www.ebi.ac.uk/swo/license/SWO_1000001"/>
        <obo:IAO_0000115>CC BY-ND 4.0 is a nonfree license, as there are restrictions on distributing modified versions. You must give appropriate credit, provide a link to the license, and indicate if changes were made. You may do so in any reasonable manner, but not in any way that suggests the licensor endorses you or your use. If you remix, transform, or build upon the material, you may not distribute the modified material. This license is generally used for documentation.</obo:IAO_0000115>
        <obo:IAO_0000118>Creative Commons Attribution-NoDerivatives 4.0 International (CC BY-ND 4.0)</obo:IAO_0000118>
        <obo:IAO_0000119>https://www.gnu.org/licenses/license-list.html accessed 29 June 2016; https://creativecommons.org/licenses/by-nd/3.0/ accessed 29 June 2016.</obo:IAO_0000119>
        <dc:creator>Allyson Lister</dc:creator>
        <rdfs:label xml:lang="en">CC BY-ND 4.0</rdfs:label>
    </owl:Class>
    


    <!-- http://www.ebi.ac.uk/swo/license/SWO_1000079 -->

    <owl:Class rdf:about="http://www.ebi.ac.uk/swo/license/SWO_1000079">
        <rdfs:subClassOf rdf:resource="http://www.ebi.ac.uk/swo/license/SWO_1000001"/>
        <rdfs:subClassOf rdf:resource="http://www.ebi.ac.uk/swo/license/SWO_1000140"/>
        <obo:IAO_0000115>CC BY-NC 3.0 is a nonfree license, as there are restrictions on charging money for copies. You must give appropriate credit, provide a link to the license, use the work for non-commercial purposes, and indicate if changes were made. You may do so in any reasonable manner, but not in any way that suggests the licensor endorses you or your use. The GNU Project does not recommend that you use this license for documentation. In addition, it has a drawback for any sort of work: when a modified version has many authors, in practice getting permission for commercial use from all of them would become infeasible.

</obo:IAO_0000115>
        <obo:IAO_0000118>Creative Commons Attribution-NonCommercial 3.0 Unported (CC BY-NC 3.0)</obo:IAO_0000118>
        <obo:IAO_0000119>https://www.gnu.org/licenses/license-list.html accessed 29 June 2016.</obo:IAO_0000119>
        <dc:creator>Allyson Lister</dc:creator>
        <rdfs:label xml:lang="en">CC BY-NC 3.0</rdfs:label>
    </owl:Class>
    


    <!-- http://www.ebi.ac.uk/swo/license/SWO_1000080 -->

    <owl:Class rdf:about="http://www.ebi.ac.uk/swo/license/SWO_1000080">
        <rdfs:subClassOf rdf:resource="http://www.ebi.ac.uk/swo/license/SWO_1000001"/>
        <rdfs:subClassOf rdf:resource="http://www.ebi.ac.uk/swo/license/SWO_1000140"/>
        <obo:IAO_0000115>CC BY-NC 4.0 is a nonfree license, as there are restrictions on charging money for copies. You must give appropriate credit, provide a link to the license, use the work for non-commercial purposes, and indicate if changes were made. You may do so in any reasonable manner, but not in any way that suggests the licensor endorses you or your use. The GNU Project does not recommend that you use this license for documentation. In addition, it has a drawback for any sort of work: when a modified version has many authors, in practice getting permission for commercial use from all of them would become infeasible.

</obo:IAO_0000115>
        <obo:IAO_0000118>Creative Commons Attribution-NonCommercial 4.0 International (CC BY-NC 4.0)</obo:IAO_0000118>
        <obo:IAO_0000119>https://www.gnu.org/licenses/license-list.html accessed 29 June 2016.</obo:IAO_0000119>
        <dc:creator>Allyson Lister</dc:creator>
        <rdfs:label>CC BY-NC 4.0</rdfs:label>
    </owl:Class>
    


    <!-- http://www.ebi.ac.uk/swo/license/SWO_1000081 -->

    <owl:Class rdf:about="http://www.ebi.ac.uk/swo/license/SWO_1000081">
        <rdfs:subClassOf rdf:resource="http://www.ebi.ac.uk/swo/license/SWO_1000001"/>
        <rdfs:subClassOf rdf:resource="http://www.ebi.ac.uk/swo/license/SWO_1000140"/>
        <obo:IAO_0000115>CC BY-NC-ND 3.0 is a nonfree license, as there are restrictions on distributing modified versions and on charging money for copies. You must give appropriate credit, provide a link to the license, and use the work for non-commercial purposes. You may do so in any reasonable manner, but not in any way that suggests the licensor endorses you or your use. If you remix, transform, or build upon the material, you may not distribute the modified material. </obo:IAO_0000115>
        <obo:IAO_0000118>Creative Commons Attribution-NonCommercial-NoDerivs 3.0 Unported (CC BY-NC-ND 3.0)</obo:IAO_0000118>
        <obo:IAO_0000119>https://www.gnu.org/licenses/license-list.html accessed 29 June 2016.</obo:IAO_0000119>
        <dc:creator>Allyson Lister</dc:creator>
        <rdfs:label xml:lang="en">CC BY-NC-ND 3.0</rdfs:label>
    </owl:Class>
    


    <!-- http://www.ebi.ac.uk/swo/license/SWO_1000083 -->

    <owl:Class rdf:about="http://www.ebi.ac.uk/swo/license/SWO_1000083">
        <rdfs:subClassOf rdf:resource="http://www.ebi.ac.uk/swo/license/SWO_1000001"/>
        <rdfs:subClassOf rdf:resource="http://www.ebi.ac.uk/swo/license/SWO_1000140"/>
        <obo:IAO_0000115>CC BY-NC-ND 2.5 is a nonfree license, as there are restrictions on distributing modified versions and on charging money for copies. You must give appropriate credit, provide a link to the license, and use the work for non-commercial purposes. You may do so in any reasonable manner, but not in any way that suggests the licensor endorses you or your use. If you remix, transform, or build upon the material, you may not distribute the modified material. </obo:IAO_0000115>
        <obo:IAO_0000118>Creative Commons Attribution-NonCommercial-NoDerivs 2.5 Generic (CC BY-NC-ND 2.5)</obo:IAO_0000118>
        <obo:IAO_0000119>https://www.gnu.org/licenses/license-list.html accessed 29 June 2016.</obo:IAO_0000119>
        <dc:creator>Allyson Lister</dc:creator>
        <rdfs:label xml:lang="en">CC BY-NC-ND 2.5</rdfs:label>
    </owl:Class>
    


    <!-- http://www.ebi.ac.uk/swo/license/SWO_1000084 -->

    <owl:Class rdf:about="http://www.ebi.ac.uk/swo/license/SWO_1000084">
        <rdfs:subClassOf rdf:resource="http://www.ebi.ac.uk/swo/license/SWO_1000001"/>
        <rdfs:subClassOf rdf:resource="http://www.ebi.ac.uk/swo/license/SWO_1000140"/>
        <obo:IAO_0000115>CC BY-NC-ND 2.5 CH is a nonfree license, as there are restrictions on distributing modified versions and on charging money for copies. You must give appropriate credit, provide a link to the license, and use the work for non-commercial purposes. You may do so in any reasonable manner, but not in any way that suggests the licensor endorses you or your use. If you remix, transform, or build upon the material, you may not distribute the modified material. </obo:IAO_0000115>
        <obo:IAO_0000118>Creative Commons Attribution-NonCommercial-NoDerivs 2.5 Switzerland (CC BY-NC-ND 2.5 CH)</obo:IAO_0000118>
        <obo:IAO_0000119>https://www.gnu.org/licenses/license-list.html accessed 29 June 2016.</obo:IAO_0000119>
        <dc:creator>Allyson Lister</dc:creator>
        <rdfs:label xml:lang="en">CC BY-NC-ND 2.5 CH</rdfs:label>
    </owl:Class>
    


    <!-- http://www.ebi.ac.uk/swo/license/SWO_1000085 -->

    <owl:Class rdf:about="http://www.ebi.ac.uk/swo/license/SWO_1000085">
        <rdfs:subClassOf rdf:resource="http://www.ebi.ac.uk/swo/license/SWO_1000001"/>
        <rdfs:subClassOf rdf:resource="http://www.ebi.ac.uk/swo/license/SWO_1000140"/>
        <obo:IAO_0000115>CC BY-NC-ND 4.0 is a nonfree license, as there are restrictions on distributing modified versions and on charging money for copies. You must give appropriate credit, provide a link to the license, and use the work for non-commercial purposes. You may do so in any reasonable manner, but not in any way that suggests the licensor endorses you or your use. If you remix, transform, or build upon the material, you may not distribute the modified material. </obo:IAO_0000115>
        <obo:IAO_0000118>Creative Commons Attribution-NonCommercial-NoDerivs 4.0 International (CC BY-NC-ND 4.0)</obo:IAO_0000118>
        <obo:IAO_0000119>https://www.gnu.org/licenses/license-list.html accessed 29 June 2016.</obo:IAO_0000119>
        <dc:creator>Allyson Lister</dc:creator>
        <rdfs:label xml:lang="en">CC BY-NC-ND 4.0</rdfs:label>
    </owl:Class>
    


    <!-- http://www.ebi.ac.uk/swo/license/SWO_1000086 -->

    <owl:Class rdf:about="http://www.ebi.ac.uk/swo/license/SWO_1000086">
        <rdfs:subClassOf rdf:resource="http://www.ebi.ac.uk/swo/license/SWO_1000001"/>
        <rdfs:subClassOf rdf:resource="http://www.ebi.ac.uk/swo/license/SWO_1000140"/>
        <obo:IAO_0000115>CC BY-NC-SA 2.5 is a nonfree license, as there are restrictions on charging money for copies. You must give appropriate credit, provide a link to the license, and indicate if changes were made. You may do so in any reasonable manner, but not in any way that suggests the licensor endorses you or your use. This license also lets others build upon the original work for non-commercial purposes, as long as they credit you and license their new creations under the identical terms. The GNU Project does not recommend that you use this license for documentation. In addition, it has a drawback for any sort of work: when a modified version has many authors, in practice getting permission for commercial use from all of them would become infeasible.

</obo:IAO_0000115>
        <obo:IAO_0000118>Creative Commons Attribution-NonCommercial-ShareAlike 2.5 Generic (CC BY-NC-SA 2.5)</obo:IAO_0000118>
        <obo:IAO_0000119>https://www.gnu.org/licenses/license-list.html accessed 29 June 2016.</obo:IAO_0000119>
        <dc:creator>Allyson Lister</dc:creator>
        <rdfs:label xml:lang="en">CC BY-NC-SA 2.5</rdfs:label>
    </owl:Class>
    


    <!-- http://www.ebi.ac.uk/swo/license/SWO_1000087 -->

    <owl:Class rdf:about="http://www.ebi.ac.uk/swo/license/SWO_1000087">
        <rdfs:subClassOf rdf:resource="http://www.ebi.ac.uk/swo/license/SWO_1000001"/>
        <rdfs:subClassOf rdf:resource="http://www.ebi.ac.uk/swo/license/SWO_1000140"/>
        <obo:IAO_0000115>CC BY-NC-SA 3.0 is a nonfree license, as there are restrictions on charging money for copies. You must give appropriate credit, provide a link to the license, and indicate if changes were made. You may do so in any reasonable manner, but not in any way that suggests the licensor endorses you or your use. This license also lets others build upon the original work for non-commercial purposes, as long as they credit you and license their new creations under the identical terms. The GNU Project does not recommend that you use this license for documentation. In addition, it has a drawback for any sort of work: when a modified version has many authors, in practice getting permission for commercial use from all of them would become infeasible.

</obo:IAO_0000115>
        <obo:IAO_0000118>Creative Commons Attribution-NonCommercial-ShareAlike 3.0 Unported (CC BY-NC-SA 3.0)</obo:IAO_0000118>
        <obo:IAO_0000119>https://www.gnu.org/licenses/license-list.html accessed 29 June 2016.</obo:IAO_0000119>
        <dc:creator>Allyson Lister</dc:creator>
        <rdfs:label xml:lang="en">CC BY-NC-SA 3.0</rdfs:label>
    </owl:Class>
    


    <!-- http://www.ebi.ac.uk/swo/license/SWO_1000088 -->

    <owl:Class rdf:about="http://www.ebi.ac.uk/swo/license/SWO_1000088">
        <rdfs:subClassOf rdf:resource="http://www.ebi.ac.uk/swo/license/SWO_1000001"/>
        <rdfs:subClassOf rdf:resource="http://www.ebi.ac.uk/swo/license/SWO_1000140"/>
        <obo:IAO_0000115>CC BY-NC-SA 3.0 US is a nonfree license, as there are restrictions on charging money for copies. You must give appropriate credit, provide a link to the license, and indicate if changes were made. You may do so in any reasonable manner, but not in any way that suggests the licensor endorses you or your use. This license also lets others build upon the original work for non-commercial purposes, as long as they credit you and license their new creations under the identical terms. The GNU Project does not recommend that you use this license for documentation. In addition, it has a drawback for any sort of work: when a modified version has many authors, in practice getting permission for commercial use from all of them would become infeasible.

</obo:IAO_0000115>
        <obo:IAO_0000118>Creative Commons Attribution-NonCommercial-ShareAlike 3.0 United States (CC BY-NC-SA 3.0 US)</obo:IAO_0000118>
        <obo:IAO_0000119>https://www.gnu.org/licenses/license-list.html accessed 29 June 2016.</obo:IAO_0000119>
        <dc:creator>Allyson Lister</dc:creator>
        <rdfs:label xml:lang="en">CC BY-NC-SA 3.0 US</rdfs:label>
    </owl:Class>
    


    <!-- http://www.ebi.ac.uk/swo/license/SWO_1000089 -->

    <owl:Class rdf:about="http://www.ebi.ac.uk/swo/license/SWO_1000089">
        <rdfs:subClassOf rdf:resource="http://www.ebi.ac.uk/swo/license/SWO_1000001"/>
        <rdfs:subClassOf rdf:resource="http://www.ebi.ac.uk/swo/license/SWO_1000140"/>
        <obo:IAO_0000115>CC BY-NC-SA 2.5 IN is a nonfree license, as there are restrictions on charging money for copies. You must give appropriate credit, provide a link to the license, and indicate if changes were made. You may do so in any reasonable manner, but not in any way that suggests the licensor endorses you or your use. This license also lets others build upon the original work for non-commercial purposes, as long as they credit you and license their new creations under the identical terms. The GNU Project does not recommend that you use this license for documentation. In addition, it has a drawback for any sort of work: when a modified version has many authors, in practice getting permission for commercial use from all of them would become infeasible.

</obo:IAO_0000115>
        <obo:IAO_0000118>Creative Commons Attribution-NonCommercial-ShareAlike 2.5 India (CC BY-NC-SA 2.5 IN)</obo:IAO_0000118>
        <obo:IAO_0000119>https://www.gnu.org/licenses/license-list.html accessed 29 June 2016.</obo:IAO_0000119>
        <dc:creator>Allyson Lister</dc:creator>
        <rdfs:label xml:lang="en">CC BY-NC-SA 2.5 IN</rdfs:label>
    </owl:Class>
    


    <!-- http://www.ebi.ac.uk/swo/license/SWO_1000090 -->

    <owl:Class rdf:about="http://www.ebi.ac.uk/swo/license/SWO_1000090">
        <rdfs:subClassOf rdf:resource="http://www.ebi.ac.uk/swo/license/SWO_1000001"/>
        <rdfs:subClassOf rdf:resource="http://www.ebi.ac.uk/swo/license/SWO_1000140"/>
        <obo:IAO_0000115>CC BY-NC-SA 4.0 is a nonfree license, as there are restrictions on charging money for copies. You must give appropriate credit, provide a link to the license, and indicate if changes were made. You may do so in any reasonable manner, but not in any way that suggests the licensor endorses you or your use. This license also lets others build upon the original work for non-commercial purposes, as long as they credit you and license their new creations under the identical terms. The GNU Project does not recommend that you use this license for documentation. In addition, it has a drawback for any sort of work: when a modified version has many authors, in practice getting permission for commercial use from all of them would become infeasible.

</obo:IAO_0000115>
        <obo:IAO_0000118>Creative Commons Attribution-NonCommercial-ShareAlike 4.0 International (CC BY-NC-SA 4.0)</obo:IAO_0000118>
        <obo:IAO_0000119>https://www.gnu.org/licenses/license-list.html accessed 29 June 2016.</obo:IAO_0000119>
        <dc:creator>Allyson Lister</dc:creator>
        <rdfs:label xml:lang="en">CC BY-NC-SA 4.0</rdfs:label>
    </owl:Class>
    


    <!-- http://www.ebi.ac.uk/swo/license/SWO_1000091 -->

    <owl:Class rdf:about="http://www.ebi.ac.uk/swo/license/SWO_1000091">
        <rdfs:subClassOf rdf:resource="http://www.ebi.ac.uk/swo/license/SWO_1000001"/>
        <rdfs:subClassOf rdf:resource="http://www.ebi.ac.uk/swo/license/SWO_1000043"/>
        <obo:IAO_0000115>CC BY-SA 2.1 JP is a copyleft free (free by the definition of the GNU Project) license which lets others remix, tweak, and build upon your work even for commercial purposes, as long as they credit you and license their new creations under the identical terms. The GNU Project recommend this license for art, entertainment and educational works, but also recommend that it is not used for software or documentation, since it is tricky as to how exactly this license is compatible with the GNU GPL.</obo:IAO_0000115>
        <obo:IAO_0000118>Creative Commons Attribution-Sharealike 2.1 Japan</obo:IAO_0000118>
        <obo:IAO_0000119>Modified from http://www.gnu.org/licenses/license-list.html, accessed 12 June 2013; Modified from http://creativecommons.org/licenses/, accessed 12 June 2013.</obo:IAO_0000119>
        <dc:creator>Allyson Lister</dc:creator>
        <rdfs:label>CC BY-SA 2.1 JP</rdfs:label>
    </owl:Class>
    


    <!-- http://www.ebi.ac.uk/swo/license/SWO_1000092 -->

    <owl:Class rdf:about="http://www.ebi.ac.uk/swo/license/SWO_1000092">
        <rdfs:subClassOf rdf:resource="http://www.ebi.ac.uk/swo/license/SWO_1000001"/>
        <rdfs:subClassOf rdf:resource="http://www.ebi.ac.uk/swo/license/SWO_1000043"/>
        <obo:IAO_0000115>CC BY-SA 3.0 is a copyleft free (free by the definition of the GNU Project) license which lets others remix, tweak, and build upon your work even for commercial purposes, as long as they credit you and license their new creations under the identical terms. The GNU Project recommend this license for art, entertainment and educational works, but also recommend that it is not used for software or documentation, since it is tricky as to how exactly this license is compatible with the GNU GPL.</obo:IAO_0000115>
        <obo:IAO_0000118>Creative Commons Attribution-Sharealike 3.0 Unported</obo:IAO_0000118>
        <obo:IAO_0000119>Modified from http://www.gnu.org/licenses/license-list.html, accessed 12 June 2013; Modified from http://creativecommons.org/licenses/, accessed 12 June 2013.</obo:IAO_0000119>
        <dc:creator>Allyson Lister</dc:creator>
        <rdfs:label xml:lang="en">CC BY-SA 3.0</rdfs:label>
    </owl:Class>
    


    <!-- http://www.ebi.ac.uk/swo/license/SWO_1000093 -->

    <owl:Class rdf:about="http://www.ebi.ac.uk/swo/license/SWO_1000093">
        <rdfs:subClassOf rdf:resource="http://www.ebi.ac.uk/swo/license/SWO_1000001"/>
        <rdfs:subClassOf rdf:resource="http://www.ebi.ac.uk/swo/license/SWO_1000043"/>
        <obo:IAO_0000115>CC BY-SA 3.0 US is a copyleft free (free by the definition of the GNU Project) license which lets others remix, tweak, and build upon your work even for commercial purposes, as long as they credit you and license their new creations under the identical terms. The GNU Project recommend this license for art, entertainment and educational works, but also recommend that it is not used for software or documentation, since it is tricky as to how exactly this license is compatible with the GNU GPL.</obo:IAO_0000115>
        <obo:IAO_0000118>Creative Commons Attribution-Sharealike 3.0 United States</obo:IAO_0000118>
        <obo:IAO_0000119>Modified from http://www.gnu.org/licenses/license-list.html, accessed 12 June 2013; Modified from http://creativecommons.org/licenses/, accessed 12 June 2013.</obo:IAO_0000119>
        <dc:creator>Allyson Lister</dc:creator>
        <rdfs:label xml:lang="en">CC BY-SA 3.0 US</rdfs:label>
    </owl:Class>
    


    <!-- http://www.ebi.ac.uk/swo/license/SWO_1000094 -->

    <owl:Class rdf:about="http://www.ebi.ac.uk/swo/license/SWO_1000094">
        <rdfs:subClassOf rdf:resource="http://www.ebi.ac.uk/swo/license/SWO_1000001"/>
        <rdfs:subClassOf rdf:resource="http://www.ebi.ac.uk/swo/license/SWO_1000043"/>
        <obo:IAO_0000115>CC BY-SA 4.0 is a copyleft free (free by the definition of the GNU Project) license which lets others remix, tweak, and build upon your work even for commercial purposes, as long as they credit you and license their new creations under the identical terms. The GNU Project recommend this license for art, entertainment and educational works, but also recommend that it is not used for software or documentation, since it is tricky as to how exactly this license is compatible with the GNU GPL.</obo:IAO_0000115>
        <obo:IAO_0000118>Creative Commons Attribution-Sharealike 4.0 International</obo:IAO_0000118>
        <obo:IAO_0000119>Modified from http://www.gnu.org/licenses/license-list.html, accessed 12 June 2013; Modified from http://creativecommons.org/licenses/, accessed 12 June 2013.</obo:IAO_0000119>
        <dc:creator>Allyson Lister</dc:creator>
        <rdfs:label xml:lang="en">CC BY-SA 4.0</rdfs:label>
    </owl:Class>
    


    <!-- http://www.ebi.ac.uk/swo/license/SWO_1000095 -->

    <owl:Class rdf:about="http://www.ebi.ac.uk/swo/license/SWO_1000095">
        <rdfs:subClassOf rdf:resource="http://www.ebi.ac.uk/swo/SWO_0000002"/>
        <rdfs:label xml:lang="en">Open Data Commons</rdfs:label>
    </owl:Class>
    


    <!-- http://www.ebi.ac.uk/swo/license/SWO_1000096 -->

    <owl:Class rdf:about="http://www.ebi.ac.uk/swo/license/SWO_1000096">
        <rdfs:subClassOf rdf:resource="http://www.ebi.ac.uk/swo/license/SWO_1000043"/>
        <rdfs:subClassOf rdf:resource="http://www.ebi.ac.uk/swo/license/SWO_1000095"/>
        <obo:IAO_0000115>The ODbL v1.0 allows a user of the databases to share, create and adapt the database. You must attribute any public use of the database, or works produced from the database. For redistribution of the database or derivative works, you must make the use of this license clear to others, and you must keep intact any notices on the original database. If you publicly use any adapted version of this database, or works produced from an adapted database, you must also offer that adapted database under the ODbL. If you redistribute the database, or an adapted version of it, then you may use technological measures that restrict the work (such as DRM) as long as you also redistribute a version without such measures.</obo:IAO_0000115>
        <obo:IAO_0000118>Open Database License (ODbL) v1.0</obo:IAO_0000118>
        <obo:IAO_0000119>http://opendatacommons.org/licenses/odbl/summary/, accessed 5 July 2016.</obo:IAO_0000119>
        <dc:creator>Allyson Lister</dc:creator>
        <rdfs:label xml:lang="en">ODbL v1.0</rdfs:label>
    </owl:Class>
    


    <!-- http://www.ebi.ac.uk/swo/license/SWO_1000097 -->

    <owl:Class rdf:about="http://www.ebi.ac.uk/swo/license/SWO_1000097">
        <rdfs:subClassOf rdf:resource="http://www.ebi.ac.uk/swo/license/SWO_1000043"/>
        <rdfs:subClassOf rdf:resource="http://www.ebi.ac.uk/swo/license/SWO_1000095"/>
        <obo:IAO_0000115>The DbCL v1.0 allows a user of the database contents to share, create and adapt the contents. You must attribute any public use of the contents, or works produced from them. For redistribution or derivative works, you must make the use of this license clear to others, and you must keep intact any notices on the original. If you publicly use any adapted version, or works produced from an adapted version, you must also offer it under the DbCL. If you redistribute the contents, or an adapted version of them, then you may use technological measures that restrict the work (such as DRM) as long as you also redistribute a version without such measures. Users of the DbCL must comply with the ODbL v1.0.</obo:IAO_0000115>
        <obo:IAO_0000118>ODC Database Contents License (DbCL) v1.0</obo:IAO_0000118>
        <obo:IAO_0000119>http://opendatacommons.org/licenses/odbl/summary/, accessed 5 July 2016; http://opendatacommons.org/licenses/dbcl/1.0/, accessed 5 July 2016.</obo:IAO_0000119>
        <dc:creator>Allyson Lister</dc:creator>
        <rdfs:label xml:lang="en">DbCL v1.0</rdfs:label>
    </owl:Class>
    


    <!-- http://www.ebi.ac.uk/swo/license/SWO_1000098 -->

    <owl:Class rdf:about="http://www.ebi.ac.uk/swo/license/SWO_1000098">
        <rdfs:subClassOf rdf:resource="http://www.ebi.ac.uk/swo/license/SWO_1000103"/>
        <obo:IAO_0000115>The EMBLEM ELM Academic LIcense was developed as the license for the ELM (Eukaryotic Linear Motif) resource. Non-commerical use is allowed under this license, an additional commercial license is also available. This license makes the Licensed Software available free of charge for the licensee,
which is a non-profit educational, academic and/or research institution. The software can only be used for academic research projects. This explicitly excludes projects which charge a fee, or projects that are done in
collaboration with a third party that is funding the research in whole or in part in exchange for commercial rights on the results and/or possible delay in publication of any relevant results to the academic community. The user and any research assistants, co-workers or other workers who may use the Software agree to not grant licenses on any software that includes the Licensed Software, alone or integrated into other software, to third parties. Modification of the Licensed Software code is prohibited without the prior written consent of EMBLEM.</obo:IAO_0000115>
        <obo:IAO_0000118>ELM Software License Agreement</obo:IAO_0000118>
        <obo:IAO_0000119>http://elm.eu.org/media/Elm_academic_license.pdf, accessed 6 July 2017; http://elm.eu.org/infos/about.html accessed 6 July 2016.</obo:IAO_0000119>
        <dc:creator>Allyson Lister</dc:creator>
        <rdfs:label xml:lang="en">EMBLEM ELM Academic License</rdfs:label>
    </owl:Class>
    


    <!-- http://www.ebi.ac.uk/swo/license/SWO_1000099 -->

    <owl:Class rdf:about="http://www.ebi.ac.uk/swo/license/SWO_1000099">
        <rdfs:subClassOf rdf:resource="http://www.ebi.ac.uk/swo/license/SWO_1000009"/>
        <rdfs:subClassOf rdf:resource="http://www.ebi.ac.uk/swo/license/SWO_1000043"/>
        <rdfs:subClassOf rdf:resource="http://www.ebi.ac.uk/swo/license/SWO_1000103"/>
        <obo:IAO_0000115>The FlowRepository Open Access Terms of Use license allows any individual to access the licensed product (originally the Flow Cytometry Data Repository) for any purpose. There are no restrictions on the use or redistribution of the data associated with this license, though it makes the statement that some data covered may also be included under more restrictive licensing.</obo:IAO_0000115>
        <obo:IAO_0000119>http://flowrepository.org/terms_of_service, accessed 6 July 2016.</obo:IAO_0000119>
        <dc:creator>Allyson Lister</dc:creator>
        <rdfs:label xml:lang="en">FlowRepository Open Access Terms of Use</rdfs:label>
    </owl:Class>
    


    <!-- http://www.ebi.ac.uk/swo/license/SWO_1000100 -->

    <owl:Class rdf:about="http://www.ebi.ac.uk/swo/license/SWO_1000100">
        <rdfs:subClassOf rdf:resource="http://www.ebi.ac.uk/swo/license/SWO_1000043"/>
        <rdfs:subClassOf rdf:resource="http://www.ebi.ac.uk/swo/license/SWO_1000095"/>
        <obo:IAO_0000115>The ODbL v1.0 allows a user of the databases to share, create and adapt the database. You must attribute any public use of the database, or works produced from the database. For redistribution of the database or derivative works, you must make the use of this license clear to others, and you must keep intact any notices on the original database. If you redistribute the database, or an adapted version of it, then you may use technological measures that restrict the work (such as DRM) as long as you also redistribute a version without such measures.</obo:IAO_0000115>
        <obo:IAO_0000118>Open Data Commons Attribution License (ODC-By) v1.0</obo:IAO_0000118>
        <obo:IAO_0000119>http://opendatacommons.org/licenses/by/summary/, accessed 6 July 2016.</obo:IAO_0000119>
        <dc:creator>Allyson Lister</dc:creator>
        <rdfs:label xml:lang="en">ODC-By v1.0</rdfs:label>
    </owl:Class>
    


    <!-- http://www.ebi.ac.uk/swo/license/SWO_1000101 -->

    <owl:Class rdf:about="http://www.ebi.ac.uk/swo/license/SWO_1000101">
        <rdfs:subClassOf rdf:resource="http://www.ebi.ac.uk/swo/license/SWO_1000009"/>
        <rdfs:subClassOf rdf:resource="http://www.ebi.ac.uk/swo/license/SWO_1000044"/>
        <rdfs:subClassOf rdf:resource="http://www.ebi.ac.uk/swo/license/SWO_1000095"/>
        <obo:IAO_0000115>The ODC Public Domain Dedication and Licence is a document intended to allow you to freely share, modify, and use this work for any purpose and without any restrictions. This licence is intended for use on databases or their contents (“data”), either together or individually. The goal is to eliminate restrictions held by the original creator of the data and database on the use of it by others. Rightsholders will not be able to “dual license” their work by releasing the same work under different licences. This is because they have allowed anyone to use the work in whatever way they choose. Rightsholders therefore can’t re-license it under copyright or database rights on different terms because they have nothing left to license. </obo:IAO_0000115>
        <obo:IAO_0000118>ODC Public Domain Dedication and Licence</obo:IAO_0000118>
        <obo:IAO_0000119>http://opendatacommons.org/licenses/pddl/1.0/, accessed 7 July 2016.</obo:IAO_0000119>
        <dc:creator>Allyson Lister</dc:creator>
        <rdfs:label xml:lang="en">PDDL v1.0</rdfs:label>
    </owl:Class>
    


    <!-- http://www.ebi.ac.uk/swo/license/SWO_1000103 -->

    <owl:Class rdf:about="http://www.ebi.ac.uk/swo/license/SWO_1000103">
        <rdfs:subClassOf rdf:resource="http://www.ebi.ac.uk/swo/SWO_0000002"/>
        <obo:IAO_0000115>A vendor-specific license is a license which was, at least originally, created by a specific organization to be used just on the resources created within that organization. This is a hierarchy of convenience rather than of shared philosophy. Many of the licenses have since been taken up by other groups whose licensing requirements matched those of the originating organization.</obo:IAO_0000115>
        <obo:IAO_0000119>Allyson Lister</obo:IAO_0000119>
        <dc:creator>Allyson Lister</dc:creator>
        <rdfs:label xml:lang="en">Vendor-specific License</rdfs:label>
    </owl:Class>
    


    <!-- http://www.ebi.ac.uk/swo/license/SWO_1000104 -->

    <owl:Class rdf:about="http://www.ebi.ac.uk/swo/license/SWO_1000104">
        <rdfs:subClassOf rdf:resource="http://www.ebi.ac.uk/swo/license/SWO_1000103"/>
        <obo:IAO_0000115>The NIDA NIH Data Access Policy specifies under what legal requirements NIDA NIH data may be accessed. Researchers may gain access to clinical data, genetic analysis data, and DNA by obtaining formal approval from the NIDA Genetic Data Access Request Committee. </obo:IAO_0000115>
        <obo:IAO_0000119>Allyson Lister</obo:IAO_0000119>
        <dc:creator>Allyson Lister</dc:creator>
        <rdfs:label xml:lang="en">NIDA NIH Data Access Policy</rdfs:label>
    </owl:Class>
    


    <!-- http://www.ebi.ac.uk/swo/license/SWO_1000105 -->

    <owl:Class rdf:about="http://www.ebi.ac.uk/swo/license/SWO_1000105">
        <rdfs:subClassOf rdf:resource="http://www.ebi.ac.uk/swo/license/SWO_1000103"/>
        <obo:IAO_0000115>The Addgene Terms of Use specifies under what legal requirements Addgene data may be accessed. Data is available for use for non-commercial purposes, but users must get express written consent of Addgene to exploit the data for commercial purposes. All copyright, trademark and other proprietary notices must be retained on the data. As consent must be aquired for commercial use, this license only allows non-commercial use (a separate agreement must be entered into for commercial use).</obo:IAO_0000115>
        <obo:IAO_0000119>https://www.addgene.org/terms-of-use/, accessed 7 July 2016</obo:IAO_0000119>
        <dc:creator>Allyson Lister</dc:creator>
        <rdfs:label xml:lang="en">Addgene Terms of Use</rdfs:label>
    </owl:Class>
    


    <!-- http://www.ebi.ac.uk/swo/license/SWO_1000106 -->

    <owl:Class rdf:about="http://www.ebi.ac.uk/swo/license/SWO_1000106">
        <rdfs:subClassOf rdf:resource="http://www.ebi.ac.uk/swo/license/SWO_1000103"/>
        <obo:IAO_0000115>The CAS Information Use Policy specifies under what legal requirements CAS Information may be accessed. Attribution to ACS must be included whenever creating derivatives or redistributing data covered under this license.Each User is permitted to download and retain a maximum of 5,000 Records and a maximum of 5,000 Molfiles at any given time for personal use or to share within a Project team for the life of the Project. There are also limits on how long records may be stored with the licensee, and how records may be linked.</obo:IAO_0000115>
        <obo:IAO_0000119>http://www.cas.org/legal/infopolicy accessed 7 July 2016.</obo:IAO_0000119>
        <dc:creator>Allyson Lister</dc:creator>
        <rdfs:label>CAS Information Use Policy</rdfs:label>
    </owl:Class>
    


    <!-- http://www.ebi.ac.uk/swo/license/SWO_1000107 -->

    <owl:Class rdf:about="http://www.ebi.ac.uk/swo/license/SWO_1000107">
        <rdfs:subClassOf rdf:resource="http://www.ebi.ac.uk/swo/license/SWO_1000103"/>
        <obo:IAO_0000115>The created contents and works provided under this license by CellFinder are subject to the German copyright law. Third-party contributions are marked as such. Reproduction, adaptation, dissemination and any kind of exploitation outside the limits of the copyright require the written consent of the author or creator. Downloads and copies of these pages are only permitted for private, non-commercial use. The operators of these pages aim to observe the copyright of others or will refer to their own or license-free works.</obo:IAO_0000115>
        <obo:IAO_0000119>http://cellfinder.de/contact/disclaimer/, accessed 7 July 2016.</obo:IAO_0000119>
        <dc:creator>Allyson Lister</dc:creator>
        <rdfs:label xml:lang="en">CellFinder Copyright</rdfs:label>
    </owl:Class>
    


    <!-- http://www.ebi.ac.uk/swo/license/SWO_1000108 -->

    <owl:Class rdf:about="http://www.ebi.ac.uk/swo/license/SWO_1000108">
        <rdfs:subClassOf rdf:resource="http://www.ebi.ac.uk/swo/license/SWO_1000103"/>
        <obo:IAO_0000115>The LINCS Data Policy is a license which allows redistribution and derivative works as long as the original data is attributed correctly. All investigators are encouraged, to publish results based on LINCS data. These results may include, but would not be limited to, integrating LINCS data with data from other sources. LINCS data are released with the sole restriction that they must be correctly cited so that others can establish provenance and access the original data; the correct citation will be released with each data set and will comprise either a PMID/PMCID reference or a unique LINCS identifier. </obo:IAO_0000115>
        <obo:IAO_0000119>http://www.lincsproject.org/data/data-release-policy/, accessed 7 July 2016.</obo:IAO_0000119>
        <dc:creator>Allyson Lister</dc:creator>
        <rdfs:label xml:lang="en">LINCS Data Policy</rdfs:label>
    </owl:Class>
    


    <!-- http://www.ebi.ac.uk/swo/license/SWO_1000109 -->

    <owl:Class rdf:about="http://www.ebi.ac.uk/swo/license/SWO_1000109">
        <rdfs:subClassOf rdf:resource="http://www.ebi.ac.uk/swo/license/SWO_1000103"/>
        <obo:IAO_0000115>The GeneNetwork Conditions of Use describes the data licensing for the resource covered. Commercial and non-commercial use is allowed, though attribution is requested via either acknowledgement or co-authorship. Further restrictions on the bulk download of as-yet unpublished data is also described. (While mentioned in the document, software licensing is not the focus of this conditions of use and therefore is not modelled here.)</obo:IAO_0000115>
        <obo:IAO_0000119>http://www.genenetwork.org/conditionsofUse.html, accessed 7 July 2016.</obo:IAO_0000119>
        <dc:creator>Allyson Lister</dc:creator>
        <rdfs:label xml:lang="en">GeneNetwork Conditions of Use</rdfs:label>
    </owl:Class>
    


    <!-- http://www.ebi.ac.uk/swo/license/SWO_1000110 -->

    <owl:Class rdf:about="http://www.ebi.ac.uk/swo/license/SWO_1000110">
        <rdfs:subClassOf rdf:resource="http://www.ebi.ac.uk/swo/license/SWO_1000103"/>
        <obo:IAO_0000115>The GMD Academic License is a vendor-specific license which allows the access and use of the licensed data for non-commercial purposes, as long as the appropriate attribution is used and copyright notices retained. A separate license agreement is required for commercial users and as such, they are not covered by this license. Without written consent by the GMD, no part of the GMD - in its original or in any way processed or reformatted form - may be re-distributed in any way.</obo:IAO_0000115>
        <obo:IAO_0000118>Golm Metabolome Database Academic License</obo:IAO_0000118>
        <obo:IAO_0000119>http://gmd.mpimp-golm.mpg.de/termsconditions.aspx, accessed 7 July 2016.</obo:IAO_0000119>
        <rdfs:label xml:lang="en">GMD Academic License</rdfs:label>
    </owl:Class>
    


    <!-- http://www.ebi.ac.uk/swo/license/SWO_1000111 -->

    <owl:Class rdf:about="http://www.ebi.ac.uk/swo/license/SWO_1000111">
        <rdfs:subClassOf rdf:resource="http://www.ebi.ac.uk/swo/license/SWO_1000103"/>
        <obo:IAO_0000115>The GeneProf Academic License is a vendor-specific license which allows the access and use of the licensed resource for non-commercial purposes.</obo:IAO_0000115>
        <obo:IAO_0000119>http://www.geneprof.org/GeneProf/terms_and_conditions.jsp, accessed 7 July 2016.</obo:IAO_0000119>
        <rdfs:label xml:lang="en">GeneProf Academic License</rdfs:label>
    </owl:Class>
    


    <!-- http://www.ebi.ac.uk/swo/license/SWO_1000112 -->

    <owl:Class rdf:about="http://www.ebi.ac.uk/swo/license/SWO_1000112">
        <rdfs:subClassOf rdf:resource="http://www.ebi.ac.uk/swo/license/SWO_1000103"/>
        <obo:IAO_0000115>The European Medicines Agency Copyright states that the Agency is the owner of copyright and other intellectual property rights for documents and other content published on their website.

Information and documents made available on the Agency&apos;s webpages are public and may be reproduced and/or distributed, totally or in part, irrespective of the means and/or the formats used, for non-commercial and commercial purposes, provided that the Agency is always acknowledged as the source of the material. Such acknowledgement must be included in each copy of the material.

Citations may be made from such material without prior permission, provided the source is always acknowledged.

The above-mentioned permissions do not apply to content supplied by third parties. Therefore, for documents where the copyright vests in a third party, permission for reproduction must be obtained from this copyright holder.</obo:IAO_0000115>
        <obo:IAO_0000119>http://www.ema.europa.eu/ema/index.jsp?curl=pages/regulation/general/general_content_000178.jsp, accessed 12 July 2016.</obo:IAO_0000119>
        <dc:creator>Allyson Lister</dc:creator>
        <rdfs:label xml:lang="en">European Medicines Agency Copyright</rdfs:label>
    </owl:Class>
    


    <!-- http://www.ebi.ac.uk/swo/license/SWO_1000113 -->

    <owl:Class rdf:about="http://www.ebi.ac.uk/swo/license/SWO_1000113">
        <rdfs:subClassOf rdf:resource="http://www.ebi.ac.uk/swo/license/SWO_1000103"/>
        <obo:IAO_0000115>miRTaBase Data License is a simple vendor license which allows academic users to make use of the data for free.</obo:IAO_0000115>
        <obo:IAO_0000119>http://mirtarbase.mbc.nctu.edu.tw/cache/download/LICENSE, accessed 12 July 2016</obo:IAO_0000119>
        <dc:creator>Allyson Lister</dc:creator>
        <rdfs:label xml:lang="en">miRTaBase Data License</rdfs:label>
    </owl:Class>
    


    <!-- http://www.ebi.ac.uk/swo/license/SWO_1000114 -->

    <owl:Class rdf:about="http://www.ebi.ac.uk/swo/license/SWO_1000114">
        <rdfs:subClassOf rdf:resource="http://www.ebi.ac.uk/swo/license/SWO_1000103"/>
        <obo:IAO_0000115>GBIF Data Sharing Agreement is a simple vendor license which allows all users to make use of the data for free, as long as the source of the data is properly attributed.</obo:IAO_0000115>
        <obo:IAO_0000119>http://www.gbif.org/terms/licences/data-sharing, accessed 12 July 2016</obo:IAO_0000119>
        <dc:creator>Allyson Lister</dc:creator>
        <rdfs:label xml:lang="en">GBIF Data Sharing Agreement</rdfs:label>
    </owl:Class>
    


    <!-- http://www.ebi.ac.uk/swo/license/SWO_1000115 -->

    <owl:Class rdf:about="http://www.ebi.ac.uk/swo/license/SWO_1000115">
        <rdfs:subClassOf rdf:resource="http://www.ebi.ac.uk/swo/license/SWO_1000043"/>
        <rdfs:subClassOf rdf:resource="http://www.ebi.ac.uk/swo/license/SWO_1000103"/>
        <obo:IAO_0000115>IUPAC/InChI-Trust InChI Licence No. 1.0 is a vendor license which allows all users to make use of the resource, including the source code, for free, as long as its source is properly attributed. It is broadly compatible with the GNU GPL v3 and v2 in that it states in the license that you can change the license from this one to the GNU GPL if you wish.</obo:IAO_0000115>
        <obo:IAO_0000118>IUPAC/InChI-Trust Licence for the International Chemical Identifier (InChI)
Software version 1.04</obo:IAO_0000118>
        <obo:IAO_0000119>http://www.inchi-trust.org/wp/wp-content/uploads/2014/06/LICENCE.pdf, accessed 12 July 2016</obo:IAO_0000119>
        <dc:creator>Allyson Lister</dc:creator>
        <rdfs:label xml:lang="en">IUPAC/InChI-Trust InChI Licence No. 1.0</rdfs:label>
    </owl:Class>
    


    <!-- http://www.ebi.ac.uk/swo/license/SWO_1000116 -->

    <owl:Class rdf:about="http://www.ebi.ac.uk/swo/license/SWO_1000116">
        <rdfs:subClassOf rdf:resource="http://www.ebi.ac.uk/swo/license/SWO_1000103"/>
        <obo:IAO_0000115>The Labome copyright makes the contents of their resource freely available for browsing. Any redistribution or reproduction of part or all of the contents in any form is prohibited other than the following: you may print or download to a local hard disk extracts for your use only, with a daily limit of 50 webpages; and you may copy the content to individual third parties for their use, but only if you acknowledge the website as the source of the material.
You may not, except with our express written permission, distribute or commercially exploit the content.</obo:IAO_0000115>
        <obo:IAO_0000119>http://www.labome.com/about/copyright.html, accessed 12 July 2016.</obo:IAO_0000119>
        <dc:creator>Allyson Lister</dc:creator>
        <rdfs:label xml:lang="en">Labome Copyright</rdfs:label>
    </owl:Class>
    


    <!-- http://www.ebi.ac.uk/swo/license/SWO_1000117 -->

    <owl:Class rdf:about="http://www.ebi.ac.uk/swo/license/SWO_1000117">
        <rdfs:subClassOf rdf:resource="http://www.ebi.ac.uk/swo/license/SWO_1000103"/>
        <obo:IAO_0000115>The CTD Legal Notice and Terms of Data Use specifies under what legal requirements the CTD data may be accessed. Data is available for use for non-commercial purposes as long as the data is properly attributed, but users must get express written consent of CTD to exploit the data for commercial purposes. As consent must be aquired for commercial use, this license only allows non-commercial use (a separate agreement must be entered into for commercial use). Additionally,You must notify CTD and describe your use of their data. For quality control purposes, you must provide CTD with periodic access to your publication of their data.</obo:IAO_0000115>
        <obo:IAO_0000118>Comparative Toxicogenomics Database Legal Notice and Terms of Use</obo:IAO_0000118>
        <obo:IAO_0000119>http://ctdbase.org/about/legal.jsp, accessed 12 July 2016</obo:IAO_0000119>
        <dc:creator>Allyson Lister</dc:creator>
        <rdfs:label xml:lang="en">CTD Legal Notice and Terms of Data Use</rdfs:label>
    </owl:Class>
    


    <!-- http://www.ebi.ac.uk/swo/license/SWO_1000118 -->

    <owl:Class rdf:about="http://www.ebi.ac.uk/swo/license/SWO_1000118">
        <rdfs:subClassOf rdf:resource="http://www.ebi.ac.uk/swo/license/SWO_1000103"/>
        <obo:IAO_0000115>LOINC RELMA Terms of Use is a vendor license which allows all users to make use of the data for free, as long as the source of the data is properly attributed. An unlimited number of copies of the licensed material may be used. </obo:IAO_0000115>
        <obo:IAO_0000119>https://loinc.org/terms-of-use/, accessed 12 July 2016</obo:IAO_0000119>
        <dc:creator>Allyson Lister</dc:creator>
        <rdfs:label xml:lang="en">LOINC RELMA Terms of Use</rdfs:label>
    </owl:Class>
    


    <!-- http://www.ebi.ac.uk/swo/license/SWO_1000119 -->

    <owl:Class rdf:about="http://www.ebi.ac.uk/swo/license/SWO_1000119">
        <rdfs:subClassOf rdf:resource="http://www.ebi.ac.uk/swo/license/SWO_1000008"/>
        <rdfs:subClassOf rdf:resource="http://www.ebi.ac.uk/swo/license/SWO_1000103"/>
        <obo:IAO_0000115>MIACA Full Copyright is a vendor-specific license which allows the document it references to be copied and furnished to others, and derivative works that comment on or otherwise explain it or assist in its implementation may be prepared, copied, published and distributed, in whole or in part, without restriction of any kind, provided that the above copyright notice and this paragraph are included on all such copies and derivative works. However, this document itself may not be modified in any way, such as by removing the copyright notice or references to the MIACA Standards Initiative or other organizations, except as needed for the purpose of developing MIACA Standards Initiative Recommendations in which case the procedures for copyrights defined in the MIACA Document process must be followed, or as required to translate it into languages other than English.</obo:IAO_0000115>
        <obo:IAO_0000119>http://miaca.sourceforge.net/copyrightNotice.txt, accessed 12 July 2016</obo:IAO_0000119>
        <dc:creator>Allyson Lister</dc:creator>
        <rdfs:label xml:lang="en">MIACA Full Copyright</rdfs:label>
    </owl:Class>
    


    <!-- http://www.ebi.ac.uk/swo/license/SWO_1000120 -->

    <owl:Class rdf:about="http://www.ebi.ac.uk/swo/license/SWO_1000120">
        <rdfs:subClassOf rdf:resource="http://www.ebi.ac.uk/swo/license/SWO_1000044"/>
        <rdfs:subClassOf rdf:resource="http://www.ebi.ac.uk/swo/license/SWO_1000103"/>
        <obo:IAO_0000115>The ORCID MIT-style license is identical to the MIT License, except for the addition of the following two clauses: 1. &quot;The above license does not apply to the branding or the &quot;look and feel&quot; of the websites located at the orcid.org URL even if elements thereof are contained in the Software.&quot;; 2. &quot;Except to provide the copyright notice required above or as allowed under ORCID Inc.&apos;s Trademark Use Policy (available at http://orcid.org, under &quot;Policies&quot;), you may not use the name of ORCID, Inc., ORCID, its marks and logo, to advertise, promote or suggest any affiliation with or endorsement by ORCID, Inc. in connection with your use of the Software.&quot;. The MIT License is is a lax, permissive non-copyleft free software license, compatible with the GNU GPL. </obo:IAO_0000115>
        <obo:IAO_0000119>https://github.com/ORCID/ORCID-Source/blob/master/LICENSE.md, accessed 12 July 2016; https://www.gnu.org/licenses/license-list.html, accessed 28 June 2016.</obo:IAO_0000119>
        <rdfs:label xml:lang="en">ORCID MIT-Style License (MIT)</rdfs:label>
    </owl:Class>
    


    <!-- http://www.ebi.ac.uk/swo/license/SWO_1000121 -->

    <owl:Class rdf:about="http://www.ebi.ac.uk/swo/license/SWO_1000121">
        <rdfs:subClassOf rdf:resource="http://www.ebi.ac.uk/swo/license/SWO_1000103"/>
        <obo:IAO_0000115>The NIH Genomic Data Sharing Policy specifies under what legal requirements NIH genomic data may be accessed. Access to human data is through a tiered model involving unrestricted- and controlled-data
access mechanisms. Requests for controlled-access data are reviewed by NIH Data Access Committees (DACs).</obo:IAO_0000115>
        <obo:IAO_0000119>https://gds.nih.gov/PDF/NIH_GDS_Policy.pdf</obo:IAO_0000119>
        <dc:creator>Allyson Lister</dc:creator>
        <rdfs:label xml:lang="en">NIH Genomic Data Sharing Policy</rdfs:label>
    </owl:Class>
    


    <!-- http://www.ebi.ac.uk/swo/license/SWO_1000122 -->

    <owl:Class rdf:about="http://www.ebi.ac.uk/swo/license/SWO_1000122">
        <rdfs:subClassOf rdf:resource="http://www.ebi.ac.uk/swo/license/SWO_1000103"/>
        <obo:IAO_0000115>The Facebase Data Access Policy specifies under what legal requirements Facebase data may be accessed. Non-sensitive data is available for use for all purposes and usages. As consent must be aquired for sensitive (or closed) data, this license only covers the use of the open data (a separate agreement must be entered into for restricted access data).</obo:IAO_0000115>
        <obo:IAO_0000119>https://www.facebase.org/methods/policies/, accessed 12 July 2016</obo:IAO_0000119>
        <dc:creator>Allyson Lister</dc:creator>
        <rdfs:label xml:lang="en">Facebase Data Access Policy</rdfs:label>
    </owl:Class>
    


    <!-- http://www.ebi.ac.uk/swo/license/SWO_1000123 -->

    <owl:Class rdf:about="http://www.ebi.ac.uk/swo/license/SWO_1000123">
        <rdfs:subClassOf rdf:resource="http://www.ebi.ac.uk/swo/license/SWO_1000103"/>
        <obo:IAO_0000115>The ORCID Terms of Use is a vendor-specific license for describing how the data in the ORCID resource may be used. ORCID data can be sublicensed, reproduced, stored, transmitted, distributed, publicly performed and publicly displayed for non-commercial and commercial uses.</obo:IAO_0000115>
        <obo:IAO_0000119>http://orcid.org/content/orcid-terms-use, accessed 12 July 2016</obo:IAO_0000119>
        <dc:creator>Allyson Lister</dc:creator>
        <rdfs:label xml:lang="en">ORCID Terms of Use</rdfs:label>
    </owl:Class>
    


    <!-- http://www.ebi.ac.uk/swo/license/SWO_1000124 -->

    <owl:Class rdf:about="http://www.ebi.ac.uk/swo/license/SWO_1000124">
        <rdfs:subClassOf rdf:resource="http://www.ebi.ac.uk/swo/license/SWO_1000103"/>
        <obo:IAO_0000115>The PPDB Academic Licens specifies under what legal requirements PPDB data may be accessed. Data is available for use for non-commercial purposes, but users must get express written consent of PPDB to exploit the data for commercial purposes. The resource will be used for teaching or not-for-profit research purposes only. The resource will not be further distributed to others. The recipient agrees to acknowledge the source of the material in any publication reporting its use. As consent must be aquired for commercial use, this license only allows non-commercial use (a separate agreement must be entered into for commercial use).</obo:IAO_0000115>
        <obo:IAO_0000118>Plant Promoter Database Academic License</obo:IAO_0000118>
        <obo:IAO_0000119>http://ppdb.agr.gifu-u.ac.jp/ppdb/cgi-bin/license.cgi, accessed 12 July 2016</obo:IAO_0000119>
        <dc:creator>Allyson Lister</dc:creator>
        <rdfs:label xml:lang="en">PPDB Academic License</rdfs:label>
    </owl:Class>
    


    <!-- http://www.ebi.ac.uk/swo/license/SWO_1000125 -->

    <owl:Class rdf:about="http://www.ebi.ac.uk/swo/license/SWO_1000125">
        <rdfs:subClassOf rdf:resource="http://www.ebi.ac.uk/swo/license/SWO_1000103"/>
        <obo:IAO_0000115>The SciCrunch Terms and Conditions specifies under what legal requirements SciCrunch data may be accessed. Broadly speaking, the site conforms, both for data and for the site documents themselves, to the CC BY 3.0 license. However, particular details for this resource (other than attribution requirements) are unclear.</obo:IAO_0000115>
        <obo:IAO_0000119>https://neuinfo.org/page/terms, accessed 12 July 2016.</obo:IAO_0000119>
        <dc:creator>Allyson Lister</dc:creator>
        <rdfs:label xml:lang="en">SciCrunch Terms and Conditions</rdfs:label>
    </owl:Class>
    


    <!-- http://www.ebi.ac.uk/swo/license/SWO_1000126 -->

    <owl:Class rdf:about="http://www.ebi.ac.uk/swo/license/SWO_1000126">
        <rdfs:subClassOf rdf:resource="http://www.ebi.ac.uk/swo/license/SWO_1000103"/>
        <rdfs:subClassOf rdf:resource="http://www.ebi.ac.uk/swo/license/SWO_1000137"/>
        <obo:IAO_0000115>The ProDom Commercial License is a vendor-specific license which allows the access and use of the licensed data for commercial purposes for a fee. Non-commercial use does not require licensing or a fee, and is covered by a separate license.</obo:IAO_0000115>
        <obo:IAO_0000119>http://prodom.prabi.fr/prodom/current/html/downcom.php, accessed 12 July 2016.</obo:IAO_0000119>
        <rdfs:label xml:lang="en">ProDom Commercial License</rdfs:label>
    </owl:Class>
    


    <!-- http://www.ebi.ac.uk/swo/license/SWO_1000127 -->

    <owl:Class rdf:about="http://www.ebi.ac.uk/swo/license/SWO_1000127">
        <rdfs:subClassOf rdf:resource="http://www.ebi.ac.uk/swo/license/SWO_1000009"/>
        <rdfs:subClassOf rdf:resource="http://www.ebi.ac.uk/swo/license/SWO_1000043"/>
        <rdfs:subClassOf rdf:resource="http://www.ebi.ac.uk/swo/license/SWO_1000103"/>
        <obo:IAO_0000115>The SBGN Open License with Attribution is a very simple statement of openness for the SBGN standard and related resources available on its website. No one—not the principal investigators, nor the SBGN Editors, nor the members of the SBGN Scientific Committee, nor the funding agencies or anyone else—owns SBGN; it is a free and open community effort that extends beyond any single group, and they view themselves only as organizers and fellow developers.</obo:IAO_0000115>
        <obo:IAO_0000118>Systems Biology Graphical Notation Open License with Attribution</obo:IAO_0000118>
        <obo:IAO_0000119>http://www.sbgn.org/About, accessed 12July 2016.</obo:IAO_0000119>
        <dc:creator>Allyson Lister</dc:creator>
        <rdfs:label xml:lang="en">SBGN Open License with Attribution</rdfs:label>
    </owl:Class>
    


    <!-- http://www.ebi.ac.uk/swo/license/SWO_1000128 -->

    <owl:Class rdf:about="http://www.ebi.ac.uk/swo/license/SWO_1000128">
        <rdfs:subClassOf rdf:resource="http://www.ebi.ac.uk/swo/license/SWO_1000009"/>
        <rdfs:subClassOf rdf:resource="http://www.ebi.ac.uk/swo/license/SWO_1000043"/>
        <rdfs:subClassOf rdf:resource="http://www.ebi.ac.uk/swo/license/SWO_1000103"/>
        <obo:IAO_0000115>The NLM Open License with Attribution is a vendor-specific license which is similar to public domain, but which requests attribution. Government information at NLM Web sites is in the public domain. Public domain information may be freely distributed and copied, but it is requested that in any subsequent use the National Library of Medicine (NLM) be given appropriate acknowledgement. When using NLM Web sites, you may encounter documents, illustrations, photographs, or other information resources contributed or licensed by private individuals, companies, or organizations that may be protected by U.S. and foreign copyright laws. Transmission or reproduction of protected items beyond that allowed by fair use as defined in the copyright laws requires the written permission of the copyright owners. Specific NLM Web sites containing protected information provide additional notification of conditions associated with its use.</obo:IAO_0000115>
        <obo:IAO_0000118>National Library of Medicine Open License with Attribution</obo:IAO_0000118>
        <obo:IAO_0000119>https://www.nlm.nih.gov/copyright.html, accessed 12 July 2016.</obo:IAO_0000119>
        <dc:creator>Allyson Lister</dc:creator>
        <rdfs:label xml:lang="en">NLM Open License with Attribution</rdfs:label>
    </owl:Class>
    


    <!-- http://www.ebi.ac.uk/swo/license/SWO_1000129 -->

    <owl:Class rdf:about="http://www.ebi.ac.uk/swo/license/SWO_1000129">
        <rdfs:subClassOf rdf:resource="http://www.ebi.ac.uk/swo/license/SWO_1000103"/>
        <obo:IAO_0000115>The RegenBase Terms of Use is a vendor-specific license which requires attribution and which does not meet the requirements for open source code, as there is a statement saying that the user will NOT translate, reverse engineer, decompile or disassemble the SYSTEM, or disclose the SYSTEM or any underlying information or technology to any third party.</obo:IAO_0000115>
        <obo:IAO_0000119>http://regenbase.org/terms-of-use.html, accessed 12 July 2016</obo:IAO_0000119>
        <dc:creator>Allyson Lister</dc:creator>
        <rdfs:label xml:lang="en">RegenBase Terms of Use</rdfs:label>
    </owl:Class>
    


    <!-- http://www.ebi.ac.uk/swo/license/SWO_1000130 -->

    <owl:Class rdf:about="http://www.ebi.ac.uk/swo/license/SWO_1000130">
        <rdfs:subClassOf rdf:resource="http://www.ebi.ac.uk/swo/license/SWO_1000103"/>
        <obo:IAO_0000115>The SABIO-RK Non-Commercial Purpose License covers use of the Database for Non-Commercial Purpose only, and appropriate attribution must be given. Non-Commercial Purpose means the use of the Database solely for internal non-commercial research and academic purposes. As consent must be aquired for commercial use, a separate agreement must be entered into for commercial use and is not covered here.</obo:IAO_0000115>
        <obo:IAO_0000119>http://sabiork.h-its.org/layouts/content/termscondition.gsp, accessed 13 July 2016</obo:IAO_0000119>
        <dc:creator>Allyson Lister</dc:creator>
        <rdfs:label xml:lang="en">SABIO-RK Non-Commercial Purpose License</rdfs:label>
    </owl:Class>
    


    <!-- http://www.ebi.ac.uk/swo/license/SWO_1000131 -->

    <owl:Class rdf:about="http://www.ebi.ac.uk/swo/license/SWO_1000131">
        <rdfs:subClassOf rdf:resource="http://www.ebi.ac.uk/swo/license/SWO_1000009"/>
        <rdfs:subClassOf rdf:resource="http://www.ebi.ac.uk/swo/license/SWO_1000043"/>
        <rdfs:subClassOf rdf:resource="http://www.ebi.ac.uk/swo/license/SWO_1000103"/>
        <obo:IAO_0000115>The Terms of Use for EMBL-EBI Services reflect EMBL-EBI’s commitment to OpenScience through its mission to provide freely available online services, databases and software relating to data contributed from life science experiments to the largest possible community. They impose no additional constraints on the use of the contributed data than those provided by the data owner.  EMBL-EBI expects attribution (e.g. in publications, services or products) for any of its online services, databases or software in accordance with good scientific practice. The expected attribution will be indicated on the appropriate web page.  </obo:IAO_0000115>
        <obo:IAO_0000119>http://www.ebi.ac.uk/about/terms-of-use, accessed 13 July 2016.</obo:IAO_0000119>
        <dc:creator>Allyson Lister</dc:creator>
        <rdfs:label xml:lang="en">Terms of Use for EMBL-EBI Services</rdfs:label>
    </owl:Class>
    


    <!-- http://www.ebi.ac.uk/swo/license/SWO_1000132 -->

    <owl:Class rdf:about="http://www.ebi.ac.uk/swo/license/SWO_1000132">
        <rdfs:subClassOf rdf:resource="http://www.ebi.ac.uk/swo/license/SWO_1000103"/>
        <obo:IAO_0000115>The UCUM Terms of Use is a vendor-specific license which allows the resource it references to be used for commercial or non-commercial purposes without restriction of any kind, provided that appropriate attribution is given. However, the resource itself may not be modified in any way. Users may make and distribute an unlimited number of copies of the Licensed Materials. Each copy thereof must include the Copyright Notice and License.</obo:IAO_0000115>
        <obo:IAO_0000118>The Unified Code for Units of Measure Terms of Use</obo:IAO_0000118>
        <obo:IAO_0000119>http://unitsofmeasure.org/trac/wiki/TermsOfUse, accessed 13 July 2016</obo:IAO_0000119>
        <dc:creator>Allyson Lister</dc:creator>
        <rdfs:label xml:lang="en">UCUM Terms of Use</rdfs:label>
    </owl:Class>
    


    <!-- http://www.ebi.ac.uk/swo/license/SWO_1000133 -->

    <owl:Class rdf:about="http://www.ebi.ac.uk/swo/license/SWO_1000133">
        <rdfs:subClassOf rdf:resource="http://www.ebi.ac.uk/swo/license/SWO_1000103"/>
        <obo:IAO_0000115>The UMLS Metathesaurus License is a vendor-specific license which allows redistribution (as part of a larger computer application) as long as the original data is attributed correctly and a summary of data use provided each year. There is no cost to use the service, and may be used both commercially and non-commercially. Users must inform the resource if it is redistributed within a computer application.</obo:IAO_0000115>
        <obo:IAO_0000119>https://uts.nlm.nih.gov/license.html, accessed 13 July 2016.</obo:IAO_0000119>
        <dc:creator>Allyson Lister</dc:creator>
        <rdfs:label xml:lang="en">UMLS Metathesaurus License</rdfs:label>
    </owl:Class>
    


    <!-- http://www.ebi.ac.uk/swo/license/SWO_1000134 -->

    <owl:Class rdf:about="http://www.ebi.ac.uk/swo/license/SWO_1000134">
        <rdfs:subClassOf rdf:resource="http://www.ebi.ac.uk/swo/license/SWO_1000103"/>
        <obo:IAO_0000115>The MHAS Data Policy is a vendor-specific license which requires that users attribute the data properly. The data is accessible free of charge to all commercial and non-commercial users. </obo:IAO_0000115>
        <obo:IAO_0000119>http://www.mhasweb.org/Data.aspx, accessed 13 July 2016.</obo:IAO_0000119>
        <dc:creator>Allyson Lister</dc:creator>
        <rdfs:label xml:lang="en">MHAS Data Policy</rdfs:label>
    </owl:Class>
    


    <!-- http://www.ebi.ac.uk/swo/license/SWO_1000135 -->

    <owl:Class rdf:about="http://www.ebi.ac.uk/swo/license/SWO_1000135">
        <rdfs:subClassOf rdf:resource="http://www.ebi.ac.uk/swo/license/SWO_1000009"/>
        <rdfs:subClassOf rdf:resource="http://www.ebi.ac.uk/swo/license/SWO_1000043"/>
        <rdfs:subClassOf rdf:resource="http://www.ebi.ac.uk/swo/license/SWO_1000103"/>
        <obo:IAO_0000115>The ALFRED Copyright is a vendor-specific license which states that the resource is freely available to the scientific community for statistical analysis, the only condition being that attribution is required.</obo:IAO_0000115>
        <obo:IAO_0000118>The ALlele FREquency Database Copyright</obo:IAO_0000118>
        <obo:IAO_0000119>https://alfred.med.yale.edu/alfred/fullcopyrightpage.asp, accessed 13 July 2016.</obo:IAO_0000119>
        <dc:creator>Allyson Lister</dc:creator>
        <rdfs:label xml:lang="en">ALFRED Copyright</rdfs:label>
    </owl:Class>
    


    <!-- http://www.ebi.ac.uk/swo/license/SWO_1000137 -->

    <owl:Class rdf:about="http://www.ebi.ac.uk/swo/license/SWO_1000137">
        <rdfs:subClassOf rdf:resource="http://www.ebi.ac.uk/swo/SWO_0000002"/>
        <obo:IAO_0000115>Fee-Based Commercial License is a license which, among its license clauses, states that commercial entities may use the resource for a fee.</obo:IAO_0000115>
        <obo:IAO_0000119>Allyson Lister</obo:IAO_0000119>
        <dc:creator>Allyson Lister</dc:creator>
        <rdfs:comment>Allyson Lister: This is a convenience class which combines multiple license clauses to create a defined class, such that any license type which meets the requirements will be inferred to fall into this category.</rdfs:comment>
        <rdfs:label xml:lang="en">Fee-Based Commercial License</rdfs:label>
    </owl:Class>
    


    <!-- http://www.ebi.ac.uk/swo/license/SWO_1000138 -->

    <owl:Class rdf:about="http://www.ebi.ac.uk/swo/license/SWO_1000138">
        <rdfs:subClassOf rdf:resource="http://www.ebi.ac.uk/swo/license/SWO_1000103"/>
        <obo:IAO_0000115>The BRENDA License is a vendor-specific license which allows access to the official website and its data free of charge. Any inclusion of BRENDA components into other data bases, or redistribution of BRENDA requires a license. To obtain commercial in-house versions please contact our distributor Biobase GmbH ( http://www.biobase-international.com). In-house versions for academic users are available from Enzymeta GmbH (http://www.enzymeta.de). The copyright of the printed version is held by Springer publishers. Users of the website may retrieve a copy of the data but must not alter the BRENDA data or charge money for a copy of it, and must not distribute any BRENDA data without prior permission of the copyright holder. As there are separate licenses for in-house versions of BRENDA, please note that this license only describes the website-accessible version of BRENDA.</obo:IAO_0000115>
        <obo:IAO_0000119>http://www.brenda-enzymes.org/copy.php, accessed 13 July 2016.</obo:IAO_0000119>
        <dc:creator>Allyson Lister</dc:creator>
        <rdfs:label xml:lang="en">BRENDA License</rdfs:label>
    </owl:Class>
    


    <!-- http://www.ebi.ac.uk/swo/license/SWO_1000139 -->

    <owl:Class rdf:about="http://www.ebi.ac.uk/swo/license/SWO_1000139">
        <rdfs:subClassOf rdf:resource="http://www.ebi.ac.uk/swo/license/SWO_1000103"/>
        <obo:IAO_0000115>The TCGA Data Use Certification is a vendor-specific license which specifies the certification which must be officially agreed to before data may be accessed. There are a number of requirements in this license including attribution, non-transferability, annual progress updates, and a number of security measures.</obo:IAO_0000115>
        <obo:IAO_0000118>The Cancer Genome Atlas Data Use Certification</obo:IAO_0000118>
        <obo:IAO_0000119>http://cancergenome.nih.gov/pdfs/Data_Use_Certv082014, accessed 13 July 2016</obo:IAO_0000119>
        <dc:creator>Allyson Lister</dc:creator>
        <rdfs:label xml:lang="en">TCGA Data Use Certification</rdfs:label>
    </owl:Class>
    


    <!-- http://www.ebi.ac.uk/swo/license/SWO_1000140 -->

    <owl:Class rdf:about="http://www.ebi.ac.uk/swo/license/SWO_1000140">
        <rdfs:subClassOf rdf:resource="http://www.ebi.ac.uk/swo/SWO_0000002"/>
        <obo:IAO_0000115>Non-Commercial No-Fee License is a license which, among its license clauses, states that non-commercial entities may use the resource without a purchase or usage cost.</obo:IAO_0000115>
        <obo:IAO_0000119>Allyson Lister</obo:IAO_0000119>
        <dc:creator>Allyson Lister</dc:creator>
        <rdfs:comment>Allyson Lister: This is a convenience class which combines multiple license clauses to create a defined class, such that any license type which meets the requirements will be inferred to fall into this category.</rdfs:comment>
        <rdfs:label xml:lang="en">Non-Commercial No-Fee License</rdfs:label>
    </owl:Class>
    


    <!-- http://www.ebi.ac.uk/swo/license/SWO_1000141 -->

    <owl:Class rdf:about="http://www.ebi.ac.uk/swo/license/SWO_1000141">
        <rdfs:subClassOf rdf:resource="http://www.ebi.ac.uk/swo/license/SWO_1000103"/>
        <obo:IAO_0000115>DrugBank is offered to the public as a freely available resource. Use and re-distribution of the data, in whole or in part, for commercial purposes (including internal use) requires a license. We ask that users who download significant portions of the database cite the DrugBank paper in any resulting publications. As consent must be aquired for commercial use, this license only describes the non-commercial aspects of data usage (a separate agreement must be entered into for commercial use).</obo:IAO_0000115>
        <obo:IAO_0000119>http://www.drugbank.ca/about, accessed 13 July 2016</obo:IAO_0000119>
        <dc:creator>Allyson Lister</dc:creator>
        <rdfs:label xml:lang="en">DrugBank Academic License</rdfs:label>
    </owl:Class>
    


    <!-- http://www.ebi.ac.uk/swo/license/SWO_1000142 -->

    <owl:Class rdf:about="http://www.ebi.ac.uk/swo/license/SWO_1000142">
        <rdfs:subClassOf rdf:resource="http://www.ebi.ac.uk/swo/license/SWO_1000103"/>
        <rdfs:subClassOf rdf:resource="http://www.ebi.ac.uk/swo/license/SWO_1000137"/>
        <obo:IAO_0000115>The UCSC Genome Browser Commercial Software License is a vendor-specific license which allows the access and use of the licensed data for commercial purposes under specific restrictions for a fee. The licensee shall not have the right to create Derivative Works of the Licensed Products, and the Licensee shall not have the right to sublicense, sell, transfer, or assign the Licensed Products. Non-commercial use does not require licensing or a fee, and is covered by a separate license.</obo:IAO_0000115>
        <obo:IAO_0000119>http://genome.cse.ucsc.edu/license/gblicense.pdf, accessed 13 July 2016.</obo:IAO_0000119>
        <rdfs:label xml:lang="en">UCSC Genome Browser Commercial Software License</rdfs:label>
    </owl:Class>
    


    <!-- http://www.ebi.ac.uk/swo/license/SWO_1000145 -->

    <owl:Class rdf:about="http://www.ebi.ac.uk/swo/license/SWO_1000145">
        <rdfs:subClassOf rdf:resource="http://www.ebi.ac.uk/swo/license/SWO_1000103"/>
        <obo:IAO_0000115>Data are to be used only for purposes of research and education. Commercial use is prohibited without written permission from Xenbase.
The contributor(s) of unpublished data should be explicitly acknowledged in any publication that incorporates, or is based in part or entirely on these data. Xenbase should be explicitly acknowledged when data used in any publication, has been in part or solely derived from analysis of data from this website. As consent must be aquired for commercial use, this license only describes the non-commercial aspects of data usage (a separate agreement must be entered into for commercial use).</obo:IAO_0000115>
        <obo:IAO_0000119>http://www.xenbase.org/other/static/aboutXenbase.jsp, accessed 13 July 2016</obo:IAO_0000119>
        <dc:creator>Allyson Lister</dc:creator>
        <rdfs:label xml:lang="en">Xenbase Academic Conditions of Use</rdfs:label>
    </owl:Class>
    


    <!-- http://www.ebi.ac.uk/swo/license/SWO_1000146 -->

    <owl:Class rdf:about="http://www.ebi.ac.uk/swo/license/SWO_1000146">
        <rdfs:subClassOf rdf:resource="http://www.ebi.ac.uk/swo/license/SWO_1000103"/>
        <obo:IAO_0000115>The RIKEN copyright is a vendor-specific license which states that all text, photographs, diagrams, and other materials on their website are copyrighted by RIKEN unless explicitly specified otherwise on the website. It is prohibited to use, reproduce, or modify any of the material without RIKEN&apos;s permission.</obo:IAO_0000115>
        <obo:IAO_0000119>http://www.riken.jp/en/terms/, accessed 14 July 2016</obo:IAO_0000119>
        <dc:creator>Allyson Lister</dc:creator>
        <rdfs:label xml:lang="en">RIKEN Copyright</rdfs:label>
    </owl:Class>
    


    <!-- http://www.ebi.ac.uk/swo/license/SWO_1000147 -->

    <owl:Class rdf:about="http://www.ebi.ac.uk/swo/license/SWO_1000147">
        <rdfs:subClassOf rdf:resource="http://www.ebi.ac.uk/swo/license/SWO_1000043"/>
        <obo:IAO_0000115>The Design Science License is a license intended to be a general &quot;copyleft&quot; that can be applied to any kind of work that has protection under copyright. This license states those certain conditions under which a work published under its terms may be copied, distributed, and modified. Unlike other open source licenses, the DSL was intended to be used on any type of copyrightable work, including documentation and source code. It was the first &quot;generalized copyleft&quot; license. This is a free and copyleft license meant for general data. THe GNU Project does not recommend it for software or documentation, since it is incompatible with the GNU GPL and with the GNU FDL; however, they consider it appropriate for other kinds of data. The DSL was written by Michael Stutz. The DSL came out in the 1990s, before the formation of the Creative Commons. According to Wikipedia, once the Creative Commons arrived, Stutz considered the DSL experiment &quot;over&quot; and no longer recommended its use.</obo:IAO_0000115>
        <obo:IAO_0000119>https://www.gnu.org/licenses/dsl.html, accessed 13 July 2016; https://www.gnu.org/licenses/license-list.html, accessed 13 July 2016; https://en.wikipedia.org/wiki/Design_science_license, accessed 13 July 2016.</obo:IAO_0000119>
        <dc:creator>Allyson Lister</dc:creator>
        <rdfs:label xml:lang="en">Design Science License</rdfs:label>
    </owl:Class>
    


    <!-- http://www.ebi.ac.uk/swo/license/SWO_1000148 -->

    <owl:Class rdf:about="http://www.ebi.ac.uk/swo/license/SWO_1000148">
        <rdfs:subClassOf rdf:resource="http://www.ebi.ac.uk/swo/license/SWO_1000103"/>
        <obo:IAO_0000115>The University of Concordia Terms of Use is a vendor-specific license which states that no document appearing on this website or any other website owned, operated or controlled by Concordia may be copied, sold, reproduced, republished, downloaded, posted, transmitted or distributed by any means with the exception of downloading or printing the contents of the site for personal, non-commercial use. This use must bear in mind that Concordia reserves its copyright and its rights to exclusivity over the material.</obo:IAO_0000115>
        <obo:IAO_0000119>http://www.concordia.ca/web/terms.html, accessed 14 July 2016</obo:IAO_0000119>
        <dc:creator>Allyson Lister</dc:creator>
        <rdfs:label xml:lang="en">University of Concordia Terms of Use</rdfs:label>
    </owl:Class>
    


    <!-- http://www.ebi.ac.uk/swo/license/SWO_1000149 -->

    <owl:Class rdf:about="http://www.ebi.ac.uk/swo/license/SWO_1000149">
        <rdfs:subClassOf rdf:resource="http://www.ebi.ac.uk/swo/license/SWO_1000043"/>
        <rdfs:subClassOf rdf:resource="http://www.ebi.ac.uk/swo/license/SWO_1000103"/>
        <obo:IAO_0000115>All OME formats and software are freely available, and all OMERO and Bio-Formats source code is available under GNU public &quot;copyleft&quot; licenses or through commercial license from Glencoe Software. FLIMfit is also now available under a GNU public &quot;copyleft&quot; license.

For questions about the GNU license refer to the Frequently Asked Questions about the GNU Licenses page.

Bio-Formats - under the terms of the GNU public &quot;copyleft&quot; license, any software package linking to Bio-Formats, either directly or indirectly, cannot be distributed unless its source code is also made available under the terms of the GPL. Some components which provide reader and writer implementations for open file formats, are released under a more permissive BSD-2 license which enables non-GPL third party software. For a complete list of which file formats are included in the BSD license, see the BSD column of the supported formats table. Developers of non-GPL software wishing to leverage Bio-Formats components not covered by the BSD license may purchase a commercial license from Glencoe Software; please contact them at bioformats@glencoesoftware.com to discuss your requirements.

The core OME Model Schema files (.XSD) use the Creative Commons Attribution 4.0 International License, and as such you are free to share or adapt them as long as you attribute the OME consortium as follows; &quot;This work is derived in part from the OME specification. Copyright (C) 2002-2016 Open Microscopy Environment&quot;. See further information about using OME-XML in your work.

This website is also covered by the Creative Commons Attribution 4.0 International License - you are free to share or adapt content as long as you credit the Open Microscopy Environment. The exception to this is the screenshots and videos which can only be used for non-commercial purposes, see Attributions below.

</obo:IAO_0000115>
        <obo:IAO_0000119>http://www.openmicroscopy.org/site/about/licensing-attribution/licensing, accessed on 23 June 2016.</obo:IAO_0000119>
        <dc:creator>Allyson Lister</dc:creator>
        <rdfs:label xml:lang="en">OME Software Conditons of Use</rdfs:label>
    </owl:Class>
    


    <!-- http://www.ebi.ac.uk/swo/license/SWO_1000150 -->

    <owl:Class rdf:about="http://www.ebi.ac.uk/swo/license/SWO_1000150">
        <rdfs:subClassOf rdf:resource="http://www.ebi.ac.uk/swo/license/SWO_1000103"/>
        <obo:IAO_0000115>The ImmPort Conditions of Use is a vendor-specific license which allows the use of ImmPort data for any legal purpose except for those prohibited elsewhere in this agreement. There are very few prohibitions, and no requirement for attribution.</obo:IAO_0000115>
        <obo:IAO_0000119>https://aspera-immport.niaid.nih.gov:9443/displayAgreement, accessed 14 July 2016</obo:IAO_0000119>
        <dc:creator>Allyson Lister</dc:creator>
        <rdfs:label xml:lang="en">ImmPort Conditions of Use</rdfs:label>
    </owl:Class>
    


    <!-- http://www.ebi.ac.uk/swo/license/SWO_9000074 -->

    <owl:Class rdf:about="http://www.ebi.ac.uk/swo/license/SWO_9000074">
        <rdfs:subClassOf rdf:resource="http://www.ebi.ac.uk/swo/license/SWO_1000044"/>
        <obo:IAO_0000115>This is a lax, permissive non-copyleft free software license, compatible with the GNU GPL. It is sometimes ambiguously referred to as the MIT License.

For substantial programs it is better to use the Apache 2.0 license since it blocks patent treachery.</obo:IAO_0000115>
        <obo:IAO_0000118>Expat License</obo:IAO_0000118>
        <obo:IAO_0000119>https://www.gnu.org/licenses/license-list.html, accessed 28 June 2016.</obo:IAO_0000119>
        <rdfs:label>MIT License</rdfs:label>
    </owl:Class>
    


    <!-- http://www.ebi.ac.uk/swo/license/SWO_9000080 -->

    <owl:Class rdf:about="http://www.ebi.ac.uk/swo/license/SWO_9000080">
        <rdfs:subClassOf rdf:resource="http://www.ebi.ac.uk/swo/license/SWO_1000009"/>
        <rdfs:subClassOf rdf:resource="http://www.ebi.ac.uk/swo/license/SWO_1000043"/>
        <obo:IAO_0000115>The GNU Lesser General Public License (LGPL) is a free software license published by the Free Software Foundation (FSF). The license allows developers and companies to use and integrate LGPL software into their own (even proprietary) software without being required by the terms of a strong copyleft license to release the source code of their own software-parts. The license requires that only the LGPL software-parts be modifiable by end-users via source code availability. </obo:IAO_0000115>
        <obo:IAO_0000118>GNU Lesser General Public License</obo:IAO_0000118>
        <obo:IAO_0000119>http://en.wikipedia.org/wiki/GNU_Lesser_General_Public_License, accessed 27 March 2015.</obo:IAO_0000119>
        <dc:contributor>Allyson Lister</dc:contributor>
        <rdfs:label>GNU LGPL</rdfs:label>
    </owl:Class>
    


    <!-- http://www.ebi.ac.uk/swo/license/SWO_9000082 -->

    <owl:Class rdf:about="http://www.ebi.ac.uk/swo/license/SWO_9000082">
        <rdfs:subClassOf rdf:resource="http://www.ebi.ac.uk/swo/license/SWO_1000056"/>
        <obo:IAO_0000115>The Artistic License v1.0 is not considered a free software license by the definition of the GNU Project because it is too vague; some passages are &amp;quot;too clever for their own good&amp;quot;, and their meaning is not clear. The GNU Project recommends that it is not used except as part of the disjunctive license of Perl.</obo:IAO_0000115>
        <obo:IAO_0000119>http://www.gnu.org/licenses/license-list.html, accessed 13 June 2013.</obo:IAO_0000119>
        <dc:creator>Allyson Lister</dc:creator>
        <dc:creator>Andy Brown</dc:creator>
        <rdfs:label>Artistic License 1.0</rdfs:label>
    </owl:Class>
    


    <!-- http://www.ebi.ac.uk/swo/license/SWO_9000084 -->

    <owl:Class rdf:about="http://www.ebi.ac.uk/swo/license/SWO_9000084">
        <rdfs:subClassOf rdf:resource="http://www.ebi.ac.uk/swo/license/SWO_1000043"/>
        <obo:IAO_0000115>The Eclipse Public License is similar to the Common Public License. This is a free software license. Unfortunately, its weak copyleft and choice of law clause make it incompatible with the GNU GPL. The only change is that the EPL removes the broader patent retaliation language regarding patent infringement suits specifically against Contributors to the EPL&apos;d program.</obo:IAO_0000115>
        <obo:IAO_0000118>Eclipse Public License Version 1.0</obo:IAO_0000118>
        <obo:IAO_0000119>https://www.gnu.org/licenses/license-list.html, accessed 28 June 2016.</obo:IAO_0000119>
        <rdfs:label>EPL v1</rdfs:label>
    </owl:Class>
    


    <!-- http://www.ebi.ac.uk/swo/license/SWO_9000085 -->

    <owl:Class rdf:about="http://www.ebi.ac.uk/swo/license/SWO_9000085">
        <rdfs:subClassOf rdf:resource="http://www.ebi.ac.uk/swo/license/SWO_1000044"/>
        <obo:IAO_0000115>The Modified BSD is a software license based on he original FreeBSD license, modified by removal of the advertising clause. It is a lax, permissive non-copyleft free software license, compatible with the GNU GPL.

This license is sometimes referred to as the 3-clause BSD license.

According to the GNU Project, the modified BSD license is not bad, as lax permissive licenses go, though the Apache 2.0 license is preferable. However, it is risky to recommend use of “the BSD license”, even for special cases such as small programs, because confusion could easily occur and lead to use of the flawed original BSD license. To avoid this risk, you can suggest the X11 license instead. The X11 license and the modified BSD license are more or less equivalent.

According to the GNU project, the Apache 2.0 license is better for substantial programs, since it prevents patent treachery.</obo:IAO_0000115>
        <obo:IAO_0000118>3 clause BSD License</obo:IAO_0000118>
        <obo:IAO_0000119>http://www.gnu.org/licenses/license-list.html, accessed June 12, 2013.</obo:IAO_0000119>
        <dc:creator>Allyson Lister</dc:creator>
        <dc:creator>Andy Jones</dc:creator>
        <rdfs:label>Modified BSD</rdfs:label>
    </owl:Class>
    


    <!-- http://www.ebi.ac.uk/swo/license/SWO_9000086 -->

    <owl:Class rdf:about="http://www.ebi.ac.uk/swo/license/SWO_9000086">
        <rdfs:subClassOf rdf:resource="http://www.ebi.ac.uk/swo/license/SWO_1000043"/>
        <obo:IAO_0000118>Latex Project Public License</obo:IAO_0000118>
        <rdfs:label>LPPL</rdfs:label>
    </owl:Class>
    


    <!-- http://www.ebi.ac.uk/swo/license/SWO_9000087 -->

    <owl:Class rdf:about="http://www.ebi.ac.uk/swo/license/SWO_9000087">
        <rdfs:subClassOf rdf:resource="http://www.ebi.ac.uk/swo/license/SWO_1000008"/>
        <obo:IAO_0000115>OPL v1.0 is not a free software license according to the definition of the GNU Project because it requires sending every published modified version to a specific initial developer. </obo:IAO_0000115>
        <obo:IAO_0000118>Open Public License Version 1.0</obo:IAO_0000118>
        <obo:IAO_0000119>http://www.gnu.org/licenses/license-list.html, accessed 12 June 2013.</obo:IAO_0000119>
        <rdfs:label>OPL v1.0</rdfs:label>
    </owl:Class>
    


    <!-- http://www.ebi.ac.uk/swo/license/SWO_9000088 -->

    <owl:Class rdf:about="http://www.ebi.ac.uk/swo/license/SWO_9000088">
        <rdfs:subClassOf rdf:resource="http://www.ebi.ac.uk/swo/license/SWO_1000008"/>
        <obo:IAO_0000118>Mozilla Public License</obo:IAO_0000118>
        <rdfs:label>MPL</rdfs:label>
    </owl:Class>
</rdf:RDF>



<!-- Generated by the OWL API (version 4.5.7.2018-12-02T02:23:35Z) https://github.com/owlcs/owlapi -->

